Implement unboxing structurally (cstrs as blocks version)

erasure/theories/EUnboxing.v
@@ -29,12 +29,13 @@ Equations safe_hd {A} (l : list A) (nnil : l <> nil) : A :=
 | [] | nnil := False_rect _ (nnil eq_refl)
 | hd :: _ | _nnil := hd.
 
-Section optimize.
+Definition inspect {A : Type} (x : A) : {y : A | x = y} :=
+  @exist _ (fun y => x = y) x eq_refl.
+
+Section unbox.
   Context (Σ : GlobalContextMap.t).
 
   Section Def.
-  Import TermSpineView.
-
 
   Definition unboxable (idecl : one_inductive_body) (cdecl : constructor_body) :=
     (#|idecl.(ind_ctors)| == 1) && (cdecl.(cstr_nargs) == 1).
@@ -47,7 +48,6 @@ Section optimize.
 
 
   Notation " t 'eqn:' h " := (exist t h) (only parsing, at level 12).
-  Import Equations.Prop.Logic.
 
   Opaque is_unboxable.
 
@@ -63,82 +63,49 @@ Section optimize.
     now intros [= <- <-].
   Qed.
 
-  Equations? optimize (t : term) : term
-    by wf t (fun x y : EAst.term => size x < size y) :=
-  | e with TermSpineView.view e := {
+  Equations unbox (t : term) : term :=
     | tRel i => EAst.tRel i
-    | tEvar ev args => EAst.tEvar ev (map_InP args (fun x H => optimize x))
-    | tLambda na M => EAst.tLambda na (optimize M)
-    | tApp u v napp nnil with construct_viewc u := {
-      | view_construct kn c block_args with is_unboxable kn c :=
-        { | true => optimize (safe_hd v nnil)
-          | false => mkApps (EAst.tConstruct kn c block_args) (map_InP v (fun x H => optimize x)) }
-      | view_other u nconstr =>
-        mkApps (optimize u) (map_InP v (fun x H => optimize x))
-    }
-    | tLetIn na b b' => EAst.tLetIn na (optimize b) (optimize b')
+    | tEvar ev args => EAst.tEvar ev (map unbox args)
+    | tLambda na M => EAst.tLambda na (unbox M)
+    | tApp u v => EAst.tApp (unbox u) (unbox v)
+    | tLetIn na b b' => EAst.tLetIn na (unbox b) (unbox b')
     | tCase ind c brs with inspect (is_unboxable ind.1 0) =>
-      { | true eqn:unb with inspect (get_unboxable_case_branch ind.1 brs ) := {
-          | Some (brna, bbody) eqn:heqbr => EAst.tLetIn brna (optimize c) (optimize bbody)
-          | None eqn:heqbr :=
-            let brs' := map_InP brs (fun x H => (x.1, optimize x.2)) in
-            EAst.tCase ind (optimize c) brs' }
-        | false eqn:unb :=
-            let brs' := map_InP brs (fun x H => (x.1, optimize x.2)) in
-            EAst.tCase ind (optimize c) brs' }
+      { | true eqn:unb with inspect (get_unboxable_case_branch ind.1 (map (on_snd unbox) brs)) := {
+          | Some (brna, bbody) eqn:heqbr => EAst.tLetIn brna (unbox c) bbody
+          | None eqn:heqbr := EAst.tCase ind (unbox c) (map (on_snd unbox) brs) }
+        | false eqn:unb := EAst.tCase ind (unbox c) (map (on_snd unbox) brs) }
     | tProj p c with inspect (is_unboxable p.(proj_ind) 0) := {
-        | true eqn:unb => optimize c
-        | false eqn:unb => EAst.tProj p (optimize c) }
-    | tConstruct ind n args => EAst.tConstruct ind n args
+        | true eqn:unb => unbox c
+        | false eqn:unb => EAst.tProj p (unbox c) }
+    | tConstruct ind n args with inspect (is_unboxable ind n) => {
+       unbox (tConstruct ind n [a]) (true eqn:unb) => unbox a ;
+       unbox (tConstruct ind n args) isunb => tConstruct ind n (map unbox args) }
     | tFix mfix idx =>
-      let mfix' := map_InP mfix (fun d H => {| dname := dname d; dbody := optimize d.(dbody); rarg := d.(rarg) |}) in
+      let mfix' := map (map_def unbox) mfix in
       EAst.tFix mfix' idx
     | tCoFix mfix idx =>
-      let mfix' := map_InP mfix (fun d H => {| dname := dname d; dbody := optimize d.(dbody); rarg := d.(rarg) |}) in
+      let mfix' := map (map_def unbox) mfix in
       EAst.tCoFix mfix' idx
     | tBox => EAst.tBox
     | tVar n => EAst.tVar n
     | tConst n => EAst.tConst n
-    | tPrim p => EAst.tPrim (map_primIn p (fun x H => optimize x)) }.
-  Proof.
-    all:try lia.
-    all:try apply (In_size); tea.
-    - eapply (In_size id size) in H. unfold id in H.
-      change (fun x => size x) with size in *. lia.
-    - rewrite size_mkApps. destruct v; cbn => //. lia.
-    - rewrite size_mkApps.
-      eapply (In_size id size) in H. change (fun x => size (id x)) with size in H. unfold id in H.  cbn. lia.
-    - rewrite size_mkApps. destruct v => //=. lia.
-    - rewrite size_mkApps.
-      eapply (In_size id size) in H. change (fun x => size (id x)) with size in H. unfold id in H.  cbn. lia.
-    - move/get_unboxable_case_branch_spec: heqbr => -> //=. lia.
-    - eapply (In_size snd size) in H; cbn in H; lia.
-    - eapply (In_size snd size) in H; cbn in H; lia.
-    - eapply (In_size dbody size) in H; cbn in H; lia.
-    - eapply (In_size dbody size) in H; cbn in H; lia.
-    - destruct p as [? []]; cbn in H; eauto.
-      intuition auto; subst; cbn; try lia.
-      eapply (In_size id size) in H0. unfold id in H0.
-      change (fun x => size x) with size in H0. lia.
-  Qed.
-  End Def.
+    | tPrim p => EAst.tPrim (map_prim unbox p)
+    | tLazy t => EAst.tLazy (unbox t)
+    | tForce t => EAst.tForce (unbox t).
 
-  #[universes(polymorphic)] Hint Rewrite @map_primIn_spec @map_InP_spec : optimize.
+  End Def.
 
   Lemma map_repeat {A B} (f : A -> B) x n : map f (repeat x n) = repeat (f x) n.
   Proof using Type.
     now induction n; simpl; auto; rewrite IHn.
   Qed.
 
-  Lemma map_optimize_repeat_box n : map optimize (repeat tBox n) = repeat tBox n.
+  Lemma map_unbox_repeat_box n : map unbox (repeat tBox n) = repeat tBox n.
   Proof using Type. now rewrite map_repeat. Qed.
 
   Arguments eqb : simpl never.
 
-  Opaque optimize_unfold_clause_1.
-  Opaque optimize.
-  Opaque isEtaExp.
-  Opaque isEtaExp_unfold_clause_1.
+  (*
 
   Lemma closedn_mkApps k f l : closedn k (mkApps f l) = closedn k f && forallb (closedn k) l.
   Proof using Type.
@@ -147,9 +114,9 @@ Section optimize.
     - now rewrite IHl /= andb_assoc.
   Qed.
 
-  Lemma closed_optimize t k : closedn k t -> closedn k (optimize t).
+  Lemma closed_unbox t k : closedn k t -> closedn k (unbox t).
   Proof using Type Σ.
-    funelim (optimize t); simp optimize; rewrite -?optimize_equation_1; toAll; simpl;
+    revert k. induction t using EInduction.term_forall_list_ind; simp unbox; rewrite -?unbox_equation_1; toAll; simpl;
     intros; try easy;
     rewrite -> ?map_map_compose, ?compose_on_snd, ?compose_map_def, ?map_length;
     unfold test_def in *;
@@ -170,44 +137,45 @@ Section optimize.
   Hint Rewrite @forallb_InP_spec : isEtaExp.
   Transparent isEtaExp_unfold_clause_1.
 
-  Local Lemma optimize_mkApps_nonnil f v (nnil : v <> []):
+  Local Lemma unbox_mkApps_nonnil f v (nnil : v <> []):
     ~~ isApp f ->
-    optimize (mkApps f v) = match construct_viewc f with
+    unbox (mkApps f v) = match construct_viewc f with
       | view_construct kn c block_args =>
-         if is_unboxable kn c then optimize (safe_hd v nnil)
-         else mkApps (EAst.tConstruct kn c block_args) (map optimize v)
-      | view_other u nconstr => mkApps (optimize f) (map optimize v)
+         if is_unboxable kn c then unbox (safe_hd v nnil)
+         else mkApps (EAst.tConstruct kn c block_args) (map unbox v)
+      | view_other u nconstr => mkApps (unbox f) (map unbox v)
     end.
   Proof using Type.
-    intros napp. rewrite optimize_equation_1.
+  Admitted.
+    intros napp. rewrite unbox_equation_1.
     destruct (TermSpineView.view_mkApps (TermSpineView.view (mkApps f v)) napp nnil) as [hna [hv' ->]].
-    simp optimize; rewrite -optimize_equation_1.
+    simp unbox; rewrite -unbox_equation_1.
     destruct (construct_viewc f).
-    2:cbn; simp optimize => //.
-    simp optimize.
-    destruct (is_unboxable ind n) => //=. simp optimize.
+    2:cbn; simp unbox => //.
+    simp unbox.
+    destruct (is_unboxable ind n) => //=. simp unbox.
     replace (safe_hd v hv') with (safe_hd v nnil) => //.
     destruct v; cbn => //.
-    f_equal. now simp optimize.
+    f_equal. now simp unbox.
   Qed.
 
-  Lemma optimize_mkApps f v : ~~ isApp f ->
-    optimize (mkApps f v) = match construct_viewc f with
+  Lemma unbox_mkApps f v : ~~ isApp f ->
+    unbox (mkApps f v) = match construct_viewc f with
       | view_construct kn c block_args =>
         if is_unboxable kn c then
           match v with
-          | hd :: _ => optimize hd
-          | _ => mkApps (EAst.tConstruct kn c block_args) (map optimize v)
+          | hd :: _ => unbox hd
+          | _ => mkApps (EAst.tConstruct kn c block_args) (map unbox v)
           end
-        else mkApps (EAst.tConstruct kn c block_args) (map optimize v)
-      | view_other u nconstr => mkApps (optimize f) (map optimize v)
+        else mkApps (EAst.tConstruct kn c block_args) (map unbox v)
+      | view_other u nconstr => mkApps (unbox f) (map unbox v)
     end.
   Proof using Type.
     intros napp.
     destruct v using rev_case; simpl.
-    - destruct construct_viewc => //. simp optimize.
+    - destruct construct_viewc => //. simp unbox.
       destruct is_unboxable => //.
-    - rewrite (optimize_mkApps_nonnil f (v ++ [x])) => //.
+    - rewrite (unbox_mkApps_nonnil f (v ++ [x])) => //.
       destruct construct_viewc => //.
       destruct is_unboxable eqn:unb => //.
       destruct v eqn:hc => //=.
@@ -222,14 +190,14 @@ Section optimize.
     cbn. do 2 destruct nth_error => //. congruence.
   Qed.
 
-  Lemma optimize_csubst a k b :
+  Lemma unbox_csubst a k b :
     closed a ->
     isEtaExp Σ a ->
     isEtaExp Σ b ->
-    optimize (ECSubst.csubst a k b) = ECSubst.csubst (optimize a) k (optimize b).
+    unbox (ECSubst.csubst a k b) = ECSubst.csubst (unbox a) k (unbox b).
   Proof using Type.
     intros cla etaa; move cla before a. move etaa before a.
-    funelim (optimize b); cbn; simp optimize isEtaExp; rewrite -?isEtaExp_equation_1 -?optimize_equation_1; toAll; simpl;
+    funelim (unbox b); cbn; simp unbox isEtaExp; rewrite -?isEtaExp_equation_1 -?unbox_equation_1; toAll; simpl;
     intros; try easy;
     rewrite -> ?map_map_compose, ?compose_on_snd, ?compose_map_def, ?map_length;
     unfold test_def in *;
@@ -242,7 +210,7 @@ Section optimize.
       rewrite !csubst_mkApps in H1 *.
       rewrite isEtaExp_mkApps_napp // in H1.
       destruct construct_viewc.
-      * cbn. rewrite optimize_mkApps //.
+      * cbn. rewrite unbox_mkApps //.
       * move/andP: H1 => [] et ev.
         rewrite -H //.
         assert (map (csubst a k) v <> []).
@@ -260,7 +228,7 @@ Section optimize.
 
           destruct (construct_viewc t0) eqn:hc.
           { rewrite -mkApps_app /=.
-            rewrite optimize_mkApps // optimize_mkApps //.
+            rewrite unbox_mkApps // unbox_mkApps //.
             cbn -[lookup_inductive_pars].
             move/andP: H2 => [] ise hl.
             unfold isEtaExp_app in ise.
@@ -274,12 +242,12 @@ Section optimize.
             rewrite !map_map_compose.
             clear -etaa cla ev H0. solve_all. }
           { rewrite -mkApps_app.
-            rewrite optimize_mkApps //. rewrite hc.
-            rewrite optimize_mkApps // hc -mkApps_app map_app //.
+            rewrite unbox_mkApps //. rewrite hc.
+            rewrite unbox_mkApps // hc -mkApps_app map_app //.
             f_equal. f_equal.
             rewrite !map_map_compose.
             clear -etaa cla ev H0. solve_all. } }
-        { rewrite optimize_mkApps ?eqa //.
+        { rewrite unbox_mkApps ?eqa //.
           destruct (construct_viewc (csubst a k t)) eqn:eqc.
           2:{ f_equal. rewrite !map_map_compose. clear -etaa cla ev H0. solve_all. }
           simp isEtaExp in H2.
@@ -288,13 +256,13 @@ Section optimize.
           rewrite (lookup_inductive_pars_constructor_pars_args eqpars).
           assert (pars = 0). rtoProp. eapply Nat.leb_le in H2. lia.
           subst pars. rewrite skipn_0.
-          simp optimize; rewrite -optimize_equation_1.
+          simp unbox; rewrite -unbox_equation_1.
           { f_equal. rewrite !map_map_compose. clear -etaa cla ev H0. solve_all. } }
     - pose proof (etaExp_csubst _ _ k _ etaa H0).
       rewrite !csubst_mkApps /= in H1 *.
       assert (map (csubst a k) v <> []).
       { destruct v; cbn; congruence. }
-      rewrite optimize_mkApps //.
+      rewrite unbox_mkApps //.
       rewrite isEtaExp_Constructor // in H1.
       move/andP: H1. rewrite map_length. move=> [] etaapp etav.
       cbn -[lookup_inductive_pars].
@@ -310,7 +278,7 @@ Section optimize.
       rewrite !csubst_mkApps /= in H1 *.
       assert (map (csubst a k) v <> []).
       { destruct v; cbn; congruence. }
-      rewrite optimize_mkApps //.
+      rewrite unbox_mkApps //.
       rewrite isEtaExp_Constructor // in H1.
       rewrite GlobalContextMap.lookup_inductive_pars_spec in Heq.
       move/andP: H1. rewrite map_length. move=> [] etaapp etav.
@@ -320,189 +288,191 @@ Section optimize.
       now rewrite (lookup_inductive_pars_constructor_pars_args eqpars) in Heq.
   Qed.
 
-  Lemma optimize_substl s t :
+  Lemma unbox_substl s t :
     forallb (closedn 0) s ->
     forallb (isEtaExp Σ) s ->
     isEtaExp Σ t ->
-    optimize (substl s t) = substl (map optimize s) (optimize t).
+    unbox (substl s t) = substl (map unbox s) (unbox t).
   Proof using Type.
     induction s in t |- *; simpl; auto.
     move=> /andP[] cla cls /andP[] etaa etas etat.
     rewrite IHs //. now eapply etaExp_csubst. f_equal.
-    now rewrite optimize_csubst.
+    now rewrite unbox_csubst.
   Qed.
 
-  Lemma optimize_iota_red pars args br :
+  Lemma unbox_iota_red pars args br :
     forallb (closedn 0) args ->
     forallb (isEtaExp Σ) args ->
     isEtaExp Σ br.2 ->
-    optimize (EGlobalEnv.iota_red pars args br) = EGlobalEnv.iota_red pars (map optimize args) (on_snd optimize br).
+    unbox (EGlobalEnv.iota_red pars args br) = EGlobalEnv.iota_red pars (map unbox args) (on_snd unbox br).
   Proof using Type.
     intros cl etaargs etabr.
     unfold EGlobalEnv.iota_red.
-    rewrite optimize_substl //.
+    rewrite unbox_substl //.
     rewrite forallb_rev forallb_skipn //.
     rewrite forallb_rev forallb_skipn //.
     now rewrite map_rev map_skipn.
   Qed.
 
-  Lemma optimize_fix_subst mfix : EGlobalEnv.fix_subst (map (map_def optimize) mfix) = map optimize (EGlobalEnv.fix_subst mfix).
+  Lemma unbox_fix_subst mfix : EGlobalEnv.fix_subst (map (map_def unbox) mfix) = map unbox (EGlobalEnv.fix_subst mfix).
   Proof using Type.
     unfold EGlobalEnv.fix_subst.
     rewrite map_length.
     generalize #|mfix|.
     induction n; simpl; auto.
-    f_equal; auto. now simp optimize.
+    f_equal; auto. now simp unbox.
   Qed.
 
-  Lemma optimize_cofix_subst mfix : EGlobalEnv.cofix_subst (map (map_def optimize) mfix) = map optimize (EGlobalEnv.cofix_subst mfix).
+  Lemma unbox_cofix_subst mfix : EGlobalEnv.cofix_subst (map (map_def unbox) mfix) = map unbox (EGlobalEnv.cofix_subst mfix).
   Proof using Type.
     unfold EGlobalEnv.cofix_subst.
     rewrite map_length.
     generalize #|mfix|.
     induction n; simpl; auto.
-    f_equal; auto. now simp optimize.
+    f_equal; auto. now simp unbox.
   Qed.
 
-  Lemma optimize_cunfold_fix mfix idx n f :
+  Lemma unbox_cunfold_fix mfix idx n f :
     forallb (closedn 0) (fix_subst mfix) ->
     forallb (fun d =>  isLambda (dbody d) && isEtaExp Σ (dbody d)) mfix ->
     cunfold_fix mfix idx = Some (n, f) ->
-    cunfold_fix (map (map_def optimize) mfix) idx = Some (n, optimize f).
+    cunfold_fix (map (map_def unbox) mfix) idx = Some (n, unbox f).
   Proof using Type.
     intros hfix heta.
     unfold cunfold_fix.
     rewrite nth_error_map.
     destruct nth_error eqn:heq.
     intros [= <- <-] => /=. f_equal. f_equal.
-    rewrite optimize_substl //.
+    rewrite unbox_substl //.
     now apply isEtaExp_fix_subst.
     solve_all. eapply nth_error_all in heta; tea. cbn in heta.
     rtoProp; intuition auto.
-    f_equal. f_equal. apply optimize_fix_subst.
+    f_equal. f_equal. apply unbox_fix_subst.
     discriminate.
   Qed.
 
 
-  Lemma optimize_cunfold_cofix mfix idx n f :
+  Lemma unbox_cunfold_cofix mfix idx n f :
     forallb (closedn 0) (cofix_subst mfix) ->
     forallb (isEtaExp Σ ∘ dbody) mfix ->
     cunfold_cofix mfix idx = Some (n, f) ->
-    cunfold_cofix (map (map_def optimize) mfix) idx = Some (n, optimize f).
+    cunfold_cofix (map (map_def unbox) mfix) idx = Some (n, unbox f).
   Proof using Type.
     intros hcofix heta.
     unfold cunfold_cofix.
     rewrite nth_error_map.
     destruct nth_error eqn:heq.
     intros [= <- <-] => /=. f_equal.
-    rewrite optimize_substl //.
+    rewrite unbox_substl //.
     now apply isEtaExp_cofix_subst.
     solve_all. now eapply nth_error_all in heta; tea.
-    f_equal. f_equal. apply optimize_cofix_subst.
+    f_equal. f_equal. apply unbox_cofix_subst.
     discriminate.
   Qed.
 
-  Lemma optimize_nth {n l d} :
-    optimize (nth n l d) = nth n (map optimize l) (optimize d).
+  Lemma unbox_nth {n l d} :
+    unbox (nth n l d) = nth n (map unbox l) (unbox d).
   Proof using Type.
     induction l in n |- *; destruct n; simpl; auto.
   Qed.
 
-End optimize.
+  *)
 
-#[universes(polymorphic)] Global Hint Rewrite @map_primIn_spec @map_InP_spec : optimize.
+End unbox.
+
+#[universes(polymorphic)] Global Hint Rewrite @map_primIn_spec @map_InP_spec : unbox.
 Tactic Notation "simp_eta" "in" hyp(H) := simp isEtaExp in H; rewrite -?isEtaExp_equation_1 in H.
 Ltac simp_eta := simp isEtaExp; rewrite -?isEtaExp_equation_1.
-Tactic Notation "simp_optimize" "in" hyp(H) := simp optimize in H; rewrite -?optimize_equation_1 in H.
-Ltac simp_optimize := simp optimize; rewrite -?optimize_equation_1.
+Tactic Notation "simp_unbox" "in" hyp(H) := simp unbox in H; rewrite -?unbox_equation_1 in H.
+Ltac simp_unbox := simp unbox; rewrite -?unbox_equation_1.
 
-Definition optimize_constant_decl Σ cb :=
-  {| cst_body := option_map (optimize Σ) cb.(cst_body) |}.
+Definition unbox_constant_decl Σ cb :=
+  {| cst_body := option_map (unbox Σ) cb.(cst_body) |}.
 
-Definition optimize_inductive_decl idecl :=
+Definition unbox_inductive_decl idecl :=
   {| ind_finite := idecl.(ind_finite); ind_npars := 0; ind_bodies := idecl.(ind_bodies) |}.
 
-Definition optimize_decl Σ d :=
+Definition unbox_decl Σ d :=
   match d with
-  | ConstantDecl cb => ConstantDecl (optimize_constant_decl Σ cb)
-  | InductiveDecl idecl => InductiveDecl (optimize_inductive_decl idecl)
+  | ConstantDecl cb => ConstantDecl (unbox_constant_decl Σ cb)
+  | InductiveDecl idecl => InductiveDecl (unbox_inductive_decl idecl)
   end.
 
-Definition optimize_env Σ :=
-  map (on_snd (optimize_decl Σ)) Σ.(GlobalContextMap.global_decls).
+Definition unbox_env Σ :=
+  map (on_snd (unbox_decl Σ)) Σ.(GlobalContextMap.global_decls).
 
-Definition optimize_program (p : eprogram_env) : eprogram :=
-  (ERemoveParams.optimize_env p.1, ERemoveParams.optimize p.1 p.2).
+Definition unbox_program (p : eprogram_env) : eprogram :=
+  (unbox_env p.1, unbox p.1 p.2).
 
 Import EGlobalEnv.
 
-Lemma lookup_env_optimize Σ kn :
-  lookup_env (optimize_env Σ) kn =
-  option_map (optimize_decl Σ) (lookup_env Σ.(GlobalContextMap.global_decls) kn).
+Lemma lookup_env_unbox Σ kn :
+  lookup_env (unbox_env Σ) kn =
+  option_map (unbox_decl Σ) (lookup_env Σ.(GlobalContextMap.global_decls) kn).
 Proof.
-  unfold optimize_env.
+  unfold unbox_env.
   destruct Σ as [Σ map repr wf]; cbn.
   induction Σ at 2 4; simpl; auto.
   case: eqb_spec => //.
 Qed.
 
-Lemma lookup_constructor_optimize {Σ kn c} :
-  lookup_constructor (optimize_env Σ) kn c =
+Lemma lookup_constructor_unbox {Σ kn c} :
+  lookup_constructor (unbox_env Σ) kn c =
   match lookup_constructor Σ.(GlobalContextMap.global_decls) kn c with
-  | Some (mdecl, idecl, cdecl) => Some (optimize_inductive_decl mdecl, idecl, cdecl)
+  | Some (mdecl, idecl, cdecl) => Some (unbox_inductive_decl mdecl, idecl, cdecl)
   | None => None
   end.
 Proof.
   rewrite /lookup_constructor /lookup_inductive /lookup_minductive.
-  rewrite lookup_env_optimize.
+  rewrite lookup_env_unbox.
   destruct lookup_env as [[]|] => /= //.
   do 2 destruct nth_error => //.
 Qed.
 
-Lemma lookup_constructor_pars_args_optimize (Σ : GlobalContextMap.t) i n npars nargs :
+Lemma lookup_constructor_pars_args_unbox (Σ : GlobalContextMap.t) i n npars nargs :
   EGlobalEnv.lookup_constructor_pars_args Σ i n = Some (npars, nargs) ->
-  EGlobalEnv.lookup_constructor_pars_args (optimize_env Σ) i n = Some (0, nargs).
+  EGlobalEnv.lookup_constructor_pars_args (unbox_env Σ) i n = Some (0, nargs).
 Proof.
-  rewrite /EGlobalEnv.lookup_constructor_pars_args. rewrite lookup_constructor_optimize //=.
+  rewrite /EGlobalEnv.lookup_constructor_pars_args. rewrite lookup_constructor_unbox //=.
   destruct EGlobalEnv.lookup_constructor => //. destruct p as [[] ?] => //=. now intros [= <- <-].
 Qed.
 
-Lemma is_propositional_optimize (Σ : GlobalContextMap.t) ind :
+Lemma is_propositional_unbox (Σ : GlobalContextMap.t) ind :
   match inductive_isprop_and_pars Σ.(GlobalContextMap.global_decls) ind with
   | Some (prop, npars) =>
-    inductive_isprop_and_pars (optimize_env Σ) ind = Some (prop, 0)
+    inductive_isprop_and_pars (unbox_env Σ) ind = Some (prop, 0)
   | None =>
-    inductive_isprop_and_pars (optimize_env Σ) ind = None
+    inductive_isprop_and_pars (unbox_env Σ) ind = None
   end.
 Proof.
   rewrite /inductive_isprop_and_pars /lookup_inductive /lookup_minductive.
-  rewrite lookup_env_optimize.
+  rewrite lookup_env_unbox.
   destruct lookup_env; simpl; auto.
   destruct g; simpl; auto. destruct nth_error => //.
 Qed.
 
-Lemma is_propositional_cstr_optimize {Σ : GlobalContextMap.t} {ind c} :
+Lemma is_propositional_cstr_unbox {Σ : GlobalContextMap.t} {ind c} :
   match constructor_isprop_pars_decl Σ.(GlobalContextMap.global_decls) ind c with
   | Some (prop, npars, cdecl) =>
-    constructor_isprop_pars_decl (optimize_env Σ) ind c = Some (prop, 0, cdecl)
+    constructor_isprop_pars_decl (unbox_env Σ) ind c = Some (prop, 0, cdecl)
   | None =>
-  constructor_isprop_pars_decl (optimize_env Σ) ind c = None
+  constructor_isprop_pars_decl (unbox_env Σ) ind c = None
   end.
 Proof.
   rewrite /constructor_isprop_pars_decl /lookup_constructor /lookup_inductive /lookup_minductive.
-  rewrite lookup_env_optimize.
+  rewrite lookup_env_unbox.
   destruct lookup_env; simpl; auto.
   destruct g; simpl; auto. do 2 destruct nth_error => //.
 Qed.
 
-Lemma lookup_inductive_pars_optimize {efl : EEnvFlags} {Σ : GlobalContextMap.t} ind :
+Lemma lookup_inductive_pars_unbox {efl : EEnvFlags} {Σ : GlobalContextMap.t} ind :
   wf_glob Σ ->
   forall pars, lookup_inductive_pars Σ ind = Some pars ->
-  EGlobalEnv.lookup_inductive_pars (optimize_env Σ) ind = Some 0.
+  EGlobalEnv.lookup_inductive_pars (unbox_env Σ) ind = Some 0.
 Proof.
   rewrite /lookup_inductive_pars => wf pars.
   rewrite /lookup_inductive /lookup_minductive.
-  rewrite (lookup_env_optimize _ ind).
+  rewrite (lookup_env_unbox _ ind).
   destruct lookup_env as [[decl|]|] => //=.
 Qed.
 
@@ -551,9 +521,10 @@ Proof.
   now rewrite remove_last_app.
 Qed.
 
+(*
 Arguments lookup_inductive_pars_constructor_pars_args {Σ ind n pars args}.
 
-Lemma optimize_tApp {Σ : GlobalContextMap.t} f a : isEtaExp Σ f -> isEtaExp Σ a -> optimize Σ (EAst.tApp f a) = EAst.tApp (optimize Σ f) (optimize Σ a).
+Lemma unbox_tApp {Σ : GlobalContextMap.t} f a : isEtaExp Σ f -> isEtaExp Σ a -> unbox Σ (EAst.tApp f a) = EAst.tApp (unbox Σ f) (unbox Σ a).
 Proof.
   move=> etaf etaa.
   pose proof (isEtaExp_mkApps_intro _ _ [a] etaf).
@@ -564,11 +535,11 @@ Proof.
   { intros [? [? []]]. rewrite H0 /=.
     rewrite -[EAst.tApp _ _ ](mkApps_app _ _ [a]).
     move/andP: H2 => []. rewrite /isEtaExp_app.
-    rewrite !optimize_mkApps // cv.
+    rewrite !unbox_mkApps // cv.
     destruct lookup_constructor_pars_args as [[pars args]|] eqn:hl => //.
     rewrite (lookup_inductive_pars_constructor_pars_args hl).
     intros hpars etal.
-    rewrite -[EAst.tApp _ _ ](mkApps_app _ _ [optimize Σ a]).
+    rewrite -[EAst.tApp _ _ ](mkApps_app _ _ [unbox Σ a]).
     f_equal. rewrite !skipn_map !skipn_app map_app. f_equal.
     assert (pars - #|remove_last l| = 0) as ->.
     2:{ rewrite skipn_0 //. }
@@ -579,12 +550,12 @@ Proof.
     move => /andP[] /Nat.leb_le. lia. }
   { move/and4P=> [] iset isel _ _. rewrite (decompose_app_inv da).
     pose proof (decompose_app_notApp _ _ _ da).
-    rewrite optimize_mkApps //.
+    rewrite unbox_mkApps //.
     destruct (decompose_app_tApp_split _ _ _ _ da).
     rewrite cv. rewrite H0.
-    rewrite optimize_mkApps // cv.
-    rewrite -[EAst.tApp _ _ ](mkApps_app _ _ [optimize Σ a]). f_equal.
-    rewrite -[(_ ++ _)%list](map_app (optimize Σ) _ [a]).
+    rewrite unbox_mkApps // cv.
+    rewrite -[EAst.tApp _ _ ](mkApps_app _ _ [unbox Σ a]). f_equal.
+    rewrite -[(_ ++ _)%list](map_app (unbox Σ) _ [a]).
     f_equal.
     assert (l <> []).
     { destruct l; try congruence. eapply decompose_app_inv in da. cbn in *. now subst t. }
@@ -593,23 +564,23 @@ Proof.
 Qed.
 
 Module Fast.
-  Section fastoptimize.
+  Section fastunbox.
     Context (Σ : GlobalContextMap.t).
 
-    Equations optimize (app : list term) (t : term) : term := {
-    | app, tEvar ev args => mkApps (EAst.tEvar ev (optimize_args args)) app
-    | app, tLambda na M => mkApps (EAst.tLambda na (optimize [] M)) app
-    | app, tApp u v => optimize (optimize [] v :: app) u
-    | app, tLetIn na b b' => mkApps (EAst.tLetIn na (optimize [] b) (optimize [] b')) app
+    Equations unbox (app : list term) (t : term) : term := {
+    | app, tEvar ev args => mkApps (EAst.tEvar ev (unbox_args args)) app
+    | app, tLambda na M => mkApps (EAst.tLambda na (unbox [] M)) app
+    | app, tApp u v => unbox (unbox [] v :: app) u
+    | app, tLetIn na b b' => mkApps (EAst.tLetIn na (unbox [] b) (unbox [] b')) app
     | app, tCase ind c brs =>
-        let brs' := optimize_brs brs in
-        mkApps (EAst.tCase (ind.1, 0) (optimize [] c) brs') app
-    | app, tProj p c => mkApps (EAst.tProj {| proj_ind := p.(proj_ind); proj_npars := 0; proj_arg := p.(proj_arg) |} (optimize [] c)) app
+        let brs' := unbox_brs brs in
+        mkApps (EAst.tCase (ind.1, 0) (unbox [] c) brs') app
+    | app, tProj p c => mkApps (EAst.tProj {| proj_ind := p.(proj_ind); proj_npars := 0; proj_arg := p.(proj_arg) |} (unbox [] c)) app
     | app, tFix mfix idx =>
-        let mfix' := optimize_defs mfix in
+        let mfix' := unbox_defs mfix in
         mkApps (EAst.tFix mfix' idx) app
     | app, tCoFix mfix idx =>
-        let mfix' := optimize_defs mfix in
+        let mfix' := unbox_defs mfix in
         mkApps (EAst.tCoFix mfix' idx) app
     | app, tConstruct kn c block_args with GlobalContextMap.lookup_inductive_pars Σ (inductive_mind kn) := {
         | Some npars => mkApps (EAst.tConstruct kn c block_args) (List.skipn npars app)
@@ -617,21 +588,21 @@ Module Fast.
     | app, tPrim (primInt; primIntModel i) => mkApps (tPrim (primInt; primIntModel i)) app
     | app, tPrim (primFloat; primFloatModel f) => mkApps (tPrim (primFloat; primFloatModel f)) app
     | app, tPrim (primArray; primArrayModel a) =>
-      mkApps (tPrim (primArray; primArrayModel {| array_default := optimize [] a.(array_default); array_value := optimize_args a.(array_value) |})) app
+      mkApps (tPrim (primArray; primArrayModel {| array_default := unbox [] a.(array_default); array_value := unbox_args a.(array_value) |})) app
     | app, x => mkApps x app }
 
-    where optimize_args (t : list term) : list term :=
+    where unbox_args (t : list term) : list term :=
     { | [] := []
-      | a :: args := (optimize [] a) :: optimize_args args
+      | a :: args := (unbox [] a) :: unbox_args args
     }
 
-    where optimize_brs (t : list (list BasicAst.name × term)) : list (list BasicAst.name × term) :=
+    where unbox_brs (t : list (list BasicAst.name × term)) : list (list BasicAst.name × term) :=
     { | [] := []
-      | a :: args := (a.1, (optimize [] a.2)) :: optimize_brs args }
+      | a :: args := (a.1, (unbox [] a.2)) :: unbox_brs args }
 
-    where optimize_defs (t : mfixpoint term) : mfixpoint term :=
+    where unbox_defs (t : mfixpoint term) : mfixpoint term :=
     { | [] := []
-      | d :: defs := {| dname := dname d; dbody := optimize [] d.(dbody); rarg := d.(rarg) |} :: optimize_defs defs
+      | d :: defs := {| dname := dname d; dbody := unbox [] d.(dbody); rarg := d.(rarg) |} :: unbox_defs defs
     }.
 
     Local Ltac specIH :=
@@ -639,74 +610,74 @@ Module Fast.
           | [ H : (forall args : list term, _) |- _ ] => specialize (H [] eq_refl)
           end.
 
-    Lemma optimize_acc_opt t :
-      forall args, ERemoveParams.optimize Σ (mkApps t args) = optimize (map (ERemoveParams.optimize Σ) args) t.
+    Lemma unbox_acc_opt t :
+      forall args, ERemoveParams.unbox Σ (mkApps t args) = unbox (map (ERemoveParams.unbox Σ) args) t.
     Proof using Type.
       intros args.
-      remember (map (ERemoveParams.optimize Σ) args) as args'.
+      remember (map (ERemoveParams.unbox Σ) args) as args'.
       revert args Heqargs'.
-      set (P:= fun args' t fs => forall args, args' = map (ERemoveParams.optimize Σ) args -> ERemoveParams.optimize Σ (mkApps t args) = fs).
-      apply (optimize_elim P
-        (fun l l' => map (ERemoveParams.optimize Σ) l = l')
-        (fun l l' => map (on_snd (ERemoveParams.optimize Σ)) l = l')
-        (fun l l' => map (map_def (ERemoveParams.optimize Σ)) l = l')); subst P; cbn -[GlobalContextMap.lookup_inductive_pars isEtaExp ERemoveParams.optimize]; clear.
+      set (P:= fun args' t fs => forall args, args' = map (ERemoveParams.unbox Σ) args -> ERemoveParams.unbox Σ (mkApps t args) = fs).
+      apply (unbox_elim P
+        (fun l l' => map (ERemoveParams.unbox Σ) l = l')
+        (fun l l' => map (on_snd (ERemoveParams.unbox Σ)) l = l')
+        (fun l l' => map (map_def (ERemoveParams.unbox Σ)) l = l')); subst P; cbn -[GlobalContextMap.lookup_inductive_pars isEtaExp ERemoveParams.unbox]; clear.
       all: try reflexivity.
-      all: intros *; simp_eta; simp_optimize.
-      all: try solve [intros; subst; rtoProp; rewrite optimize_mkApps // /=; simp_optimize; repeat specIH; repeat (f_equal; intuition eauto)].
-      all: try solve [rewrite optimize_mkApps //].
+      all: intros *; simp_eta; simp_unbox.
+      all: try solve [intros; subst; rtoProp; rewrite unbox_mkApps // /=; simp_unbox; repeat specIH; repeat (f_equal; intuition eauto)].
+      all: try solve [rewrite unbox_mkApps //].
       - intros IHv IHu.
         specialize (IHv [] eq_refl). simpl in IHv.
         intros args ->. specialize (IHu (v :: args)).
         forward IHu. now rewrite -IHv. exact IHu.
       - intros Hl hargs args ->.
-        rewrite optimize_mkApps //=. simp_optimize.
+        rewrite unbox_mkApps //=. simp_unbox.
         f_equal. f_equal. cbn.
         do 2 f_equal. rewrite /map_array_model.
         specialize (Hl [] eq_refl). f_equal; eauto.
       - intros Hl args ->.
-        rewrite optimize_mkApps // /=.
+        rewrite unbox_mkApps // /=.
         rewrite GlobalContextMap.lookup_inductive_pars_spec in Hl. now rewrite Hl.
       - intros Hl args ->.
         rewrite GlobalContextMap.lookup_inductive_pars_spec in Hl.
-        now rewrite optimize_mkApps // /= Hl.
+        now rewrite unbox_mkApps // /= Hl.
       - intros IHa heq.
         specIH. now rewrite IHa.
       - intros IHa heq; specIH. f_equal; eauto. unfold on_snd. now rewrite IHa.
       - intros IHa heq; specIH. unfold map_def. f_equal; eauto. now rewrite IHa.
     Qed.
 
-    Lemma optimize_fast t : ERemoveParams.optimize Σ t = optimize [] t.
-    Proof using Type. now apply (optimize_acc_opt t []). Qed.
+    Lemma unbox_fast t : ERemoveParams.unbox Σ t = unbox [] t.
+    Proof using Type. now apply (unbox_acc_opt t []). Qed.
 
-  End fastoptimize.
+  End fastunbox.
 
-  Notation optimize' Σ := (optimize Σ []).
+  Notation unbox' Σ := (unbox Σ []).
 
-  Definition optimize_constant_decl Σ cb :=
-    {| cst_body := option_map (optimize' Σ) cb.(cst_body) |}.
+  Definition unbox_constant_decl Σ cb :=
+    {| cst_body := option_map (unbox' Σ) cb.(cst_body) |}.
 
-  Definition optimize_inductive_decl idecl :=
+  Definition unbox_inductive_decl idecl :=
     {| ind_finite := idecl.(ind_finite); ind_npars := 0; ind_bodies := idecl.(ind_bodies) |}.
 
-  Definition optimize_decl Σ d :=
+  Definition unbox_decl Σ d :=
     match d with
-    | ConstantDecl cb => ConstantDecl (optimize_constant_decl Σ cb)
-    | InductiveDecl idecl => InductiveDecl (optimize_inductive_decl idecl)
+    | ConstantDecl cb => ConstantDecl (unbox_constant_decl Σ cb)
+    | InductiveDecl idecl => InductiveDecl (unbox_inductive_decl idecl)
     end.
 
-  Definition optimize_env Σ :=
-    map (on_snd (optimize_decl Σ)) Σ.(GlobalContextMap.global_decls).
+  Definition unbox_env Σ :=
+    map (on_snd (unbox_decl Σ)) Σ.(GlobalContextMap.global_decls).
 
-  Lemma optimize_env_fast Σ : ERemoveParams.optimize_env Σ = optimize_env Σ.
+  Lemma unbox_env_fast Σ : ERemoveParams.unbox_env Σ = unbox_env Σ.
   Proof.
-    unfold ERemoveParams.optimize_env, optimize_env.
+    unfold ERemoveParams.unbox_env, unbox_env.
     destruct Σ as [Σ map repr wf]. cbn.
     induction Σ at 2 4; cbn; auto.
     f_equal; eauto.
     destruct a as [kn []]; cbn; auto.
     destruct c as [[b|]]; cbn; auto. unfold on_snd; cbn.
-    do 2 f_equal. unfold ERemoveParams.optimize_constant_decl, optimize_constant_decl.
-    simpl. f_equal. f_equal. apply optimize_fast.
+    do 2 f_equal. unfold ERemoveParams.unbox_constant_decl, unbox_constant_decl.
+    simpl. f_equal. f_equal. apply unbox_fast.
   Qed.
 
 End Fast.
@@ -756,19 +727,19 @@ Proof.
   rewrite mkApps_app /= //.
 Qed.
 
-Lemma optimize_isLambda Σ f :
-  EAst.isLambda f = EAst.isLambda (optimize Σ f).
+Lemma unbox_isLambda Σ f :
+  EAst.isLambda f = EAst.isLambda (unbox Σ f).
 Proof.
-  funelim (optimize Σ f); cbn -[optimize]; (try simp_optimize) => //.
+  funelim (unbox Σ f); cbn -[unbox]; (try simp_unbox) => //.
   rewrite (negbTE (isLambda_mkApps' _ _ _)) //.
   rewrite (negbTE (isLambda_mkApps' _ _ _)) //; try apply map_nil => //.
   all:rewrite !(negbTE (isLambda_mkApps_Construct _ _ _ _)) //.
 Qed.
 
-Lemma optimize_isBox Σ f :
-  isBox f = isBox (optimize Σ f).
+Lemma unbox_isBox Σ f :
+  isBox f = isBox (unbox Σ f).
 Proof.
-  funelim (optimize Σ f); cbn -[optimize] => //.
+  funelim (unbox Σ f); cbn -[unbox] => //.
   all:rewrite map_InP_spec.
   rewrite (negbTE (isBox_mkApps' _ _ _)) //.
   rewrite (negbTE (isBox_mkApps' _ _ _)) //; try apply map_nil => //.
@@ -781,45 +752,45 @@ Proof.
   rewrite mkApps_app /= //.
 Qed.
 
-Lemma optimize_isApp Σ f :
+Lemma unbox_isApp Σ f :
   ~~ EAst.isApp f ->
-  ~~ EAst.isApp (optimize Σ f).
+  ~~ EAst.isApp (unbox Σ f).
 Proof.
-  funelim (optimize Σ f); cbn -[optimize] => //.
+  funelim (unbox Σ f); cbn -[unbox] => //.
   all:rewrite map_InP_spec.
   all:rewrite isApp_mkApps //.
 Qed.
 
-Lemma optimize_isFix Σ f :
-  isFix f = isFix (optimize Σ f).
+Lemma unbox_isFix Σ f :
+  isFix f = isFix (unbox Σ f).
 Proof.
-  funelim (optimize Σ f); cbn -[optimize] => //.
+  funelim (unbox Σ f); cbn -[unbox] => //.
   all:rewrite map_InP_spec.
   rewrite (negbTE (isFix_mkApps' _ _ _)) //.
   rewrite (negbTE (isFix_mkApps' _ _ _)) //; try apply map_nil => //.
   all:rewrite !(negbTE (isFix_mkApps_Construct _ _ _ _)) //.
 Qed.
 
-Lemma optimize_isFixApp Σ f :
-  isFixApp f = isFixApp (optimize Σ f).
+Lemma unbox_isFixApp Σ f :
+  isFixApp f = isFixApp (unbox Σ f).
 Proof.
-  funelim (optimize Σ f); cbn -[optimize] => //.
+  funelim (unbox Σ f); cbn -[unbox] => //.
   all:rewrite map_InP_spec.
   all:rewrite isFixApp_mkApps isFixApp_mkApps //.
 Qed.
 
-Lemma optimize_isConstructApp Σ f :
-  isConstructApp f = isConstructApp (optimize Σ f).
+Lemma unbox_isConstructApp Σ f :
+  isConstructApp f = isConstructApp (unbox Σ f).
 Proof.
-  funelim (optimize Σ f); cbn -[optimize] => //.
+  funelim (unbox Σ f); cbn -[unbox] => //.
   all:rewrite map_InP_spec.
   all:rewrite isConstructApp_mkApps isConstructApp_mkApps //.
 Qed.
 
-Lemma optimize_isPrimApp Σ f :
-  isPrimApp f = isPrimApp (optimize Σ f).
+Lemma unbox_isPrimApp Σ f :
+  isPrimApp f = isPrimApp (unbox Σ f).
 Proof.
-  funelim (optimize Σ f); cbn -[optimize] => //.
+  funelim (unbox Σ f); cbn -[unbox] => //.
   all:rewrite map_InP_spec.
   all:rewrite !isPrimApp_mkApps //.
 Qed.
@@ -863,9 +834,9 @@ Proof.
   destruct nth_error => //. destruct nth_error => //. congruence.
 Qed.
 
-Lemma optimize_mkApps_etaexp {Σ : GlobalContextMap.t} fn args :
+Lemma unbox_mkApps_etaexp {Σ : GlobalContextMap.t} fn args :
   isEtaExp Σ fn ->
-  optimize Σ (EAst.mkApps fn args) = EAst.mkApps (optimize Σ fn) (map (optimize Σ) args).
+  unbox Σ (EAst.mkApps fn args) = EAst.mkApps (unbox Σ fn) (map (unbox Σ) args).
 Proof.
   destruct (decompose_app fn) eqn:da.
   rewrite (decompose_app_inv da).
@@ -873,8 +844,8 @@ Proof.
   destruct construct_viewc eqn:vc.
   + move=> /andP[] hl0 etal0.
     rewrite -mkApps_app.
-    rewrite (optimize_mkApps Σ (tConstruct ind n block_args)) // /=.
-    rewrite optimize_mkApps // /=.
+    rewrite (unbox_mkApps Σ (tConstruct ind n block_args)) // /=.
+    rewrite unbox_mkApps // /=.
     unfold isEtaExp_app in hl0.
     destruct lookup_constructor_pars_args as [[pars args']|] eqn:hl => //.
     rtoProp.
@@ -884,7 +855,7 @@ Proof.
     rewrite skipn_app. len. assert (pars - #|l| = 0) by lia.
     now rewrite H1 skipn_0.
   + move=> /andP[] etat0 etal0.
-    rewrite -mkApps_app !optimize_mkApps; try now eapply decompose_app_notApp.
+    rewrite -mkApps_app !unbox_mkApps; try now eapply decompose_app_notApp.
     rewrite vc. rewrite -mkApps_app !map_app //.
 Qed.
 
@@ -919,178 +890,177 @@ Proof.
     intros; rtoProp; intuition auto; solve_all.
 Qed.
 
-Lemma optimize_eval (efl := all_env_flags) {wfl:WcbvFlags} {wcon : with_constructor_as_block = false} {Σ : GlobalContextMap.t} t v :
+Lemma unbox_eval (efl := all_env_flags) {wfl:WcbvFlags} {wcon : with_constructor_as_block = false} {Σ : GlobalContextMap.t} t v :
   isEtaExp_env Σ ->
   closed_env Σ ->
   wf_glob Σ ->
   closedn 0 t ->
   isEtaExp Σ t ->
   eval Σ t v ->
-  eval (optimize_env Σ) (optimize Σ t) (optimize Σ v).
+  eval (unbox_env Σ) (unbox Σ t) (unbox Σ v).
 Proof.
   intros etaΣ clΣ wfΣ.
   revert t v.
-  unshelve eapply (eval_preserve_mkApps_ind wfl wcon Σ (fun x y => eval (optimize_env Σ) (optimize Σ x) (optimize Σ y))
+  unshelve eapply (eval_preserve_mkApps_ind wfl wcon Σ (fun x y => eval (unbox_env Σ) (unbox Σ x) (unbox Σ y))
     (fun n x => closedn n x) (Qpres := Qpreserves_closedn Σ clΣ)) => //.
   { intros. eapply eval_closed; tea. }
   all:intros; simpl in *.
-  (* 1-15: try solve [econstructor; eauto]. *)
   all:repeat destruct_nary_times => //.
-  - rewrite optimize_tApp //.
+  - rewrite unbox_tApp //.
     econstructor; eauto.
 
-  - rewrite optimize_tApp //. simp_optimize in e1.
+  - rewrite unbox_tApp //. simp_unbox in e1.
     econstructor; eauto.
-    rewrite optimize_csubst // in e. now simp_eta in i10.
+    rewrite unbox_csubst // in e. now simp_eta in i10.
 
-  - simp_optimize.
-    rewrite optimize_csubst // in e.
+  - simp_unbox.
+    rewrite unbox_csubst // in e.
     econstructor; eauto.
 
-  - simp_optimize.
-    set (brs' := map _ brs). cbn -[optimize].
+  - simp_unbox.
+    set (brs' := map _ brs). cbn -[unbox].
     cbn in H3.
-    rewrite optimize_mkApps // /= in e0.
+    rewrite unbox_mkApps // /= in e0.
     apply constructor_isprop_pars_decl_lookup in H2 as H1'.
     rewrite H1' in e0.
-    pose proof (@is_propositional_cstr_optimize Σ ind c).
+    pose proof (@is_propositional_cstr_unbox Σ ind c).
     rewrite H2 in H1.
     econstructor; eauto.
     * rewrite nth_error_map H3 //.
     * len. cbn in H4, H5. rewrite skipn_length. lia.
-    * cbn -[optimize]. rewrite skipn_0. len.
-    * cbn -[optimize].
+    * cbn -[unbox]. rewrite skipn_0. len.
+    * cbn -[unbox].
       have etaargs : forallb (isEtaExp Σ) args.
       { rewrite isEtaExp_Constructor in i6.
         now move/andP: i6 => [] /andP[]. }
-      rewrite optimize_iota_red // in e.
+      rewrite unbox_iota_red // in e.
       rewrite closedn_mkApps in i4. now move/andP: i4.
       cbn. now eapply nth_error_forallb in H; tea.
 
   - subst brs. cbn in H4.
     rewrite andb_true_r in H4.
-    rewrite optimize_substl // in e.
+    rewrite unbox_substl // in e.
     eapply All_forallb, All_repeat => //.
     eapply All_forallb, All_repeat => //.
-    rewrite map_optimize_repeat_box in e.
-    simp_optimize. set (brs' := map _ _).
-    cbn -[optimize]. eapply eval_iota_sing => //.
-    now move: (is_propositional_optimize Σ ind); rewrite H2.
+    rewrite map_unbox_repeat_box in e.
+    simp_unbox. set (brs' := map _ _).
+    cbn -[unbox]. eapply eval_iota_sing => //.
+    now move: (is_propositional_unbox Σ ind); rewrite H2.
 
-  - rewrite optimize_tApp //.
-    rewrite optimize_mkApps // /= in e1.
-    simp_optimize in e1.
+  - rewrite unbox_tApp //.
+    rewrite unbox_mkApps // /= in e1.
+    simp_unbox in e1.
     eapply eval_fix; tea.
     * rewrite map_length.
-      eapply optimize_cunfold_fix; tea.
+      eapply unbox_cunfold_fix; tea.
       eapply closed_fix_subst. tea.
       move: i8; rewrite closedn_mkApps => /andP[] //.
       move: i10; rewrite isEtaExp_mkApps_napp // /= => /andP[] //. simp_eta.
     * move: e.
       rewrite -[tApp _ _](mkApps_app _ _ [av]).
-      rewrite -[tApp _ _](mkApps_app _ _ [optimize _ av]).
-      rewrite optimize_mkApps_etaexp // map_app //.
+      rewrite -[tApp _ _](mkApps_app _ _ [unbox _ av]).
+      rewrite unbox_mkApps_etaexp // map_app //.
 
-  - rewrite optimize_tApp //.
-    rewrite optimize_tApp //.
-    rewrite optimize_mkApps //. simpl.
-    simp_optimize. set (mfix' := map _ _). simpl.
-    rewrite optimize_mkApps // /= in e0. simp_optimize in e0.
+  - rewrite unbox_tApp //.
+    rewrite unbox_tApp //.
+    rewrite unbox_mkApps //. simpl.
+    simp_unbox. set (mfix' := map _ _). simpl.
+    rewrite unbox_mkApps // /= in e0. simp_unbox in e0.
     eapply eval_fix_value; tea.
-    eapply optimize_cunfold_fix; eauto.
+    eapply unbox_cunfold_fix; eauto.
     eapply closed_fix_subst => //.
     { move: i4.
       rewrite closedn_mkApps. now move/andP => []. }
     { move: i6. rewrite isEtaExp_mkApps_napp // /= => /andP[] //. now simp isEtaExp. }
     now rewrite map_length.
 
-  - rewrite optimize_tApp //. simp_optimize in e0.
-    simp_optimize in e1.
+  - rewrite unbox_tApp //. simp_unbox in e0.
+    simp_unbox in e1.
     eapply eval_fix'; tea.
-    eapply optimize_cunfold_fix; tea.
+    eapply unbox_cunfold_fix; tea.
     { eapply closed_fix_subst => //. }
     { simp isEtaExp in i10. }
-    rewrite optimize_tApp // in e.
+    rewrite unbox_tApp // in e.
 
-  - simp_optimize.
-    rewrite optimize_mkApps // /= in e0.
-    simp_optimize in e.
-    simp_optimize in e0.
+  - simp_unbox.
+    rewrite unbox_mkApps // /= in e0.
+    simp_unbox in e.
+    simp_unbox in e0.
     set (brs' := map _ _) in *; simpl.
     eapply eval_cofix_case; tea.
-    eapply optimize_cunfold_cofix; tea => //.
+    eapply unbox_cunfold_cofix; tea => //.
     { eapply closed_cofix_subst; tea.
       move: i5; rewrite closedn_mkApps => /andP[] //. }
     { move: i7. rewrite isEtaExp_mkApps_napp // /= => /andP[] //. now simp isEtaExp. }
-    rewrite optimize_mkApps_etaexp // in e.
+    rewrite unbox_mkApps_etaexp // in e.
 
   - destruct p as [[ind pars] arg].
-    simp_optimize.
-    simp_optimize in e.
-    rewrite optimize_mkApps // /= in e0.
-    simp_optimize in e0.
-    rewrite optimize_mkApps_etaexp // in e.
-    simp_optimize in e0.
+    simp_unbox.
+    simp_unbox in e.
+    rewrite unbox_mkApps // /= in e0.
+    simp_unbox in e0.
+    rewrite unbox_mkApps_etaexp // in e.
+    simp_unbox in e0.
     eapply eval_cofix_proj; tea.
-    eapply optimize_cunfold_cofix; tea.
+    eapply unbox_cunfold_cofix; tea.
     { eapply closed_cofix_subst; tea.
       move: i4; rewrite closedn_mkApps => /andP[] //. }
     { move: i6. rewrite isEtaExp_mkApps_napp // /= => /andP[] //. now simp isEtaExp. }
 
   - econstructor. red in H |- *.
-    rewrite lookup_env_optimize H //.
-    now rewrite /optimize_constant_decl H0.
+    rewrite lookup_env_unbox H //.
+    now rewrite /unbox_constant_decl H0.
     exact e.
 
-  - simp_optimize.
-    rewrite optimize_mkApps // /= in e0.
+  - simp_unbox.
+    rewrite unbox_mkApps // /= in e0.
     rewrite (constructor_isprop_pars_decl_lookup H2) in e0.
     eapply eval_proj; eauto.
-    move: (@is_propositional_cstr_optimize Σ p.(proj_ind) 0). now rewrite H2. simpl.
+    move: (@is_propositional_cstr_unbox Σ p.(proj_ind) 0). now rewrite H2. simpl.
     len. rewrite skipn_length. cbn in H3. lia.
     rewrite nth_error_skipn nth_error_map /= H4 //.
 
-  - simp_optimize. eapply eval_proj_prop => //.
-    move: (is_propositional_optimize Σ p.(proj_ind)); now rewrite H3.
+  - simp_unbox. eapply eval_proj_prop => //.
+    move: (is_propositional_unbox Σ p.(proj_ind)); now rewrite H3.
 
-  - rewrite !optimize_tApp //.
+  - rewrite !unbox_tApp //.
     eapply eval_app_cong; tea.
     move: H1. eapply contraNN.
-    rewrite -optimize_isLambda -optimize_isConstructApp -optimize_isFixApp -optimize_isBox -optimize_isPrimApp //.
-    rewrite -optimize_isFix //.
+    rewrite -unbox_isLambda -unbox_isConstructApp -unbox_isFixApp -unbox_isBox -unbox_isPrimApp //.
+    rewrite -unbox_isFix //.
 
-  - rewrite !optimize_mkApps // /=.
+  - rewrite !unbox_mkApps // /=.
     rewrite (lookup_constructor_lookup_inductive_pars H).
     eapply eval_mkApps_Construct; tea.
-    + rewrite lookup_constructor_optimize H //.
-    + constructor. cbn [atom]. rewrite wcon lookup_constructor_optimize H //.
+    + rewrite lookup_constructor_unbox H //.
+    + constructor. cbn [atom]. rewrite wcon lookup_constructor_unbox H //.
     + rewrite /cstr_arity /=.
       move: H0; rewrite /cstr_arity /=.
       rewrite skipn_length map_length => ->. lia.
     + cbn in H0. eapply All2_skipn, All2_map.
-      eapply All2_impl; tea; cbn -[optimize].
+      eapply All2_impl; tea; cbn -[unbox].
       intros x y []; auto.
 
-  - depelim X; simp optimize; repeat constructor.
+  - depelim X; simp unbox; repeat constructor.
     eapply All2_over_undep in a. eapply All2_Set_All2 in ev. eapply All2_All2_Set. solve_all. now destruct b.
     now destruct a0.
 
   - destruct t => //.
-    all:constructor; eauto. simp optimize.
-    cbn [atom optimize] in H |- *.
-    rewrite lookup_constructor_optimize.
+    all:constructor; eauto. simp unbox.
+    cbn [atom unbox] in H |- *.
+    rewrite lookup_constructor_unbox.
     destruct lookup_constructor eqn:hl => //. destruct p as [[] ?] => //.
 Qed.
 
 From MetaCoq.Erasure Require Import EEtaExpanded.
 
-Lemma optimize_declared_constructor {Σ : GlobalContextMap.t} {k mdecl idecl cdecl} :
+Lemma unbox_declared_constructor {Σ : GlobalContextMap.t} {k mdecl idecl cdecl} :
   declared_constructor Σ.(GlobalContextMap.global_decls)  k mdecl idecl cdecl ->
-  declared_constructor (optimize_env Σ) k (optimize_inductive_decl mdecl) idecl cdecl.
+  declared_constructor (unbox_env Σ) k (unbox_inductive_decl mdecl) idecl cdecl.
 Proof.
   intros [[] ?]; do 2 split => //.
   red in H; red.
-  rewrite lookup_env_optimize H //.
+  rewrite lookup_env_unbox H //.
 Qed.
 
 Lemma lookup_inductive_pars_spec {Σ} {mind} {mdecl} :
@@ -1109,80 +1079,80 @@ Definition switch_no_params (efl : EEnvFlags) :=
      |}.
 
 (* Stripping preserves well-formedness directly, not caring about eta-expansion *)
-Lemma optimize_wellformed {efl} {Σ : GlobalContextMap.t} n t :
+Lemma unbox_wellformed {efl} {Σ : GlobalContextMap.t} n t :
   cstr_as_blocks = false ->
   has_tApp ->
   @wf_glob efl Σ ->
   @wellformed efl Σ n t ->
-  @wellformed (switch_no_params efl) (optimize_env Σ) n (optimize Σ t).
+  @wellformed (switch_no_params efl) (unbox_env Σ) n (unbox Σ t).
 Proof.
   intros cab hasapp wfΣ.
   revert n.
-  funelim (optimize Σ t); try intros n.
-  all:cbn -[optimize lookup_constructor lookup_inductive]; simp_optimize; intros.
+  funelim (unbox Σ t); try intros n.
+  all:cbn -[unbox lookup_constructor lookup_inductive]; simp_unbox; intros.
   all:try solve[unfold wf_fix_gen in *; rtoProp; intuition auto; toAll; solve_all].
-  - cbn -[optimize]; simp_optimize. intros; rtoProp; intuition auto.
-    rewrite lookup_env_optimize. destruct lookup_env eqn:hl => // /=.
+  - cbn -[unbox]; simp_unbox. intros; rtoProp; intuition auto.
+    rewrite lookup_env_unbox. destruct lookup_env eqn:hl => // /=.
     destruct g => /= //. destruct (cst_body c) => //.
-  - rewrite cab in H |- *. cbn -[optimize] in *.
-    rewrite lookup_env_optimize. destruct lookup_env eqn:hl => // /=.
+  - rewrite cab in H |- *. cbn -[unbox] in *.
+    rewrite lookup_env_unbox. destruct lookup_env eqn:hl => // /=.
     destruct g eqn:hg => /= //. subst g.
     destruct nth_error => //. destruct nth_error => //.
-  - cbn -[optimize].
-    rewrite lookup_env_optimize. cbn in H1. destruct lookup_env eqn:hl => // /=.
+  - cbn -[unbox].
+    rewrite lookup_env_unbox. cbn in H1. destruct lookup_env eqn:hl => // /=.
     destruct g eqn:hg => /= //. subst g.
     destruct nth_error => //. rtoProp; intuition auto.
-    simp_optimize. toAll; solve_all.
+    simp_unbox. toAll; solve_all.
     toAll. solve_all.
-  - cbn -[optimize] in H0 |- *.
-    rewrite lookup_env_optimize. destruct lookup_env eqn:hl => // /=.
+  - cbn -[unbox] in H0 |- *.
+    rewrite lookup_env_unbox. destruct lookup_env eqn:hl => // /=.
     destruct g eqn:hg => /= //. subst g. cbn in H0. now rtoProp.
     destruct nth_error => //. all:rtoProp; intuition auto.
     destruct EAst.ind_ctors => //.
     destruct nth_error => //.
     all: eapply H; auto.
   - unfold wf_fix_gen in *. rewrite map_length. rtoProp; intuition auto. toAll; solve_all.
-    now rewrite -optimize_isLambda. toAll; solve_all.
+    now rewrite -unbox_isLambda. toAll; solve_all.
   - primProp. rtoProp; intuition eauto; solve_all_k 6.
   - move:H1; rewrite !wellformed_mkApps //. rtoProp; intuition auto.
     toAll; solve_all. toAll; solve_all.
   - move:H0; rewrite !wellformed_mkApps //. rtoProp; intuition auto.
     move: H1. cbn. rewrite cab.
-    rewrite lookup_env_optimize. destruct lookup_env eqn:hl => // /=.
+    rewrite lookup_env_unbox. destruct lookup_env eqn:hl => // /=.
     destruct g eqn:hg => /= //. subst g.
     destruct nth_error => //. destruct nth_error => //.
     toAll; solve_all. eapply All_skipn. solve_all.
   - move:H0; rewrite !wellformed_mkApps //. rtoProp; intuition auto.
     move: H1. cbn. rewrite cab.
-    rewrite lookup_env_optimize. destruct lookup_env eqn:hl => // /=.
+    rewrite lookup_env_unbox. destruct lookup_env eqn:hl => // /=.
     destruct g eqn:hg => /= //. subst g.
     destruct nth_error => //. destruct nth_error => //.
     toAll; solve_all.
 Qed.
 
-Lemma optimize_wellformed_irrel {efl : EEnvFlags} {Σ : GlobalContextMap.t} t :
+Lemma unbox_wellformed_irrel {efl : EEnvFlags} {Σ : GlobalContextMap.t} t :
   cstr_as_blocks = false ->
   wf_glob Σ ->
-  forall n, wellformed Σ n t -> wellformed (optimize_env Σ) n t.
+  forall n, wellformed Σ n t -> wellformed (unbox_env Σ) n t.
 Proof.
   intros hcstrs wfΣ. induction t using EInduction.term_forall_list_ind; cbn => //.
   all:try solve [intros; unfold wf_fix in *; rtoProp; intuition eauto; solve_all].
-  - rewrite lookup_env_optimize //.
+  - rewrite lookup_env_unbox //.
     destruct lookup_env eqn:hl => // /=.
     destruct g eqn:hg => /= //. subst g.
     destruct (cst_body c) => //.
-  - rewrite lookup_env_optimize //.
+  - rewrite lookup_env_unbox //.
     destruct lookup_env eqn:hl => // /=; intros; rtoProp; eauto.
     destruct g eqn:hg => /= //; intros; rtoProp; eauto.
     destruct cstr_as_blocks => //; repeat split; eauto.
     destruct nth_error => /= //.
     destruct nth_error => /= //.
-  - rewrite lookup_env_optimize //.
+  - rewrite lookup_env_unbox //.
     destruct lookup_env eqn:hl => // /=.
     destruct g eqn:hg => /= //. subst g.
     destruct nth_error => /= //.
     intros; rtoProp; intuition auto; solve_all.
-  - rewrite lookup_env_optimize //.
+  - rewrite lookup_env_unbox //.
     destruct lookup_env eqn:hl => // /=.
     destruct g eqn:hg => /= //.
     rewrite andb_false_r => //.
@@ -1192,44 +1162,44 @@ Proof.
     destruct nth_error => //.
 Qed.
 
-Lemma optimize_wellformed_decl_irrel {efl : EEnvFlags} {Σ : GlobalContextMap.t} d :
+Lemma unbox_wellformed_decl_irrel {efl : EEnvFlags} {Σ : GlobalContextMap.t} d :
   cstr_as_blocks = false ->
   wf_glob Σ ->
-  wf_global_decl Σ d -> wf_global_decl (optimize_env Σ) d.
+  wf_global_decl Σ d -> wf_global_decl (unbox_env Σ) d.
 Proof.
   intros hcstrs wf; destruct d => /= //.
   destruct (cst_body c) => /= //.
-  now eapply optimize_wellformed_irrel.
+  now eapply unbox_wellformed_irrel.
 Qed.
 
-Lemma optimize_decl_wf (efl := all_env_flags) {Σ : GlobalContextMap.t} :
+Lemma unbox_decl_wf (efl := all_env_flags) {Σ : GlobalContextMap.t} :
   wf_glob Σ ->
   forall d, wf_global_decl Σ d ->
-  wf_global_decl (efl := switch_no_params efl) (optimize_env Σ) (optimize_decl Σ d).
+  wf_global_decl (efl := switch_no_params efl) (unbox_env Σ) (unbox_decl Σ d).
 Proof.
   intros wf d.
   destruct d => /= //.
   destruct (cst_body c) => /= //.
-  now apply (optimize_wellformed (Σ := Σ) 0 t).
+  now apply (unbox_wellformed (Σ := Σ) 0 t).
 Qed.
 
-Lemma fresh_global_optimize_env {Σ : GlobalContextMap.t} kn :
+Lemma fresh_global_unbox_env {Σ : GlobalContextMap.t} kn :
   fresh_global kn Σ ->
-  fresh_global kn (optimize_env Σ).
+  fresh_global kn (unbox_env Σ).
 Proof.
-  unfold fresh_global. cbn. unfold optimize_env.
+  unfold fresh_global. cbn. unfold unbox_env.
   induction (GlobalContextMap.global_decls Σ); cbn; constructor; auto. cbn.
   now depelim H. depelim H. eauto.
 Qed.
 
 From MetaCoq.Erasure Require Import EProgram.
 
-Program Fixpoint optimize_env' Σ : EnvMap.fresh_globals Σ -> global_context :=
+Program Fixpoint unbox_env' Σ : EnvMap.fresh_globals Σ -> global_context :=
   match Σ with
   | [] => fun _ => []
   | hd :: tl => fun HΣ =>
     let Σg := GlobalContextMap.make tl (fresh_globals_cons_inv HΣ) in
-    on_snd (optimize_decl Σg) hd :: optimize_env' tl (fresh_globals_cons_inv HΣ)
+    on_snd (unbox_decl Σg) hd :: unbox_env' tl (fresh_globals_cons_inv HΣ)
   end.
 
 Lemma lookup_minductive_declared_minductive Σ ind mdecl :
@@ -1266,25 +1236,25 @@ Proof.
   apply lookup_minductive_declared_minductive in hl. now rewrite hl.
 Qed.
 
-Lemma optimize_extends {efl : EEnvFlags} {Σ Σ' : GlobalContextMap.t} :
+Lemma unbox_extends {efl : EEnvFlags} {Σ Σ' : GlobalContextMap.t} :
   has_tApp ->
   extends Σ Σ' -> wf_glob Σ' ->
-  forall n t, wellformed Σ n t -> optimize Σ t = optimize Σ' t.
+  forall n t, wellformed Σ n t -> unbox Σ t = unbox Σ' t.
 Proof.
   intros hasapp hext hwf n t. revert n.
-  funelim (optimize Σ t); intros ?n; simp_optimize  => /= //.
+  funelim (unbox Σ t); intros ?n; simp_unbox  => /= //.
   all:try solve [intros; unfold wf_fix in *; rtoProp; intuition auto; f_equal; auto; toAll; solve_all].
   - intros; rtoProp; intuition auto.
     move: H1; rewrite wellformed_mkApps // => /andP[] wfu wfargs.
-    rewrite optimize_mkApps // Heq /=. f_equal; eauto. toAll; solve_all.
+    rewrite unbox_mkApps // Heq /=. f_equal; eauto. toAll; solve_all.
   - rewrite wellformed_mkApps // => /andP[] wfc wfv.
-    rewrite optimize_mkApps // /=.
+    rewrite unbox_mkApps // /=.
     rewrite GlobalContextMap.lookup_inductive_pars_spec in Heq.
     eapply (extends_lookup_inductive_pars hext hwf) in Heq.
     rewrite Heq. f_equal. f_equal.
     toAll; solve_all.
   - rewrite wellformed_mkApps // => /andP[] wfc wfv.
-    rewrite optimize_mkApps // /=.
+    rewrite unbox_mkApps // /=.
     move: Heq.
     rewrite GlobalContextMap.lookup_inductive_pars_spec.
     unfold wellformed in wfc. move/andP: wfc => [] /andP[] hacc hc bargs.
@@ -1292,29 +1262,29 @@ Proof.
     unfold lookup_constructor, lookup_inductive in hc. rewrite heq /= // in hc.
 Qed.
 
-Lemma optimize_decl_extends {efl : EEnvFlags} {Σ Σ' : GlobalContextMap.t} :
+Lemma unbox_decl_extends {efl : EEnvFlags} {Σ Σ' : GlobalContextMap.t} :
   has_tApp ->
   extends Σ Σ' -> wf_glob Σ' ->
-  forall d, wf_global_decl Σ d -> optimize_decl Σ d = optimize_decl Σ' d.
+  forall d, wf_global_decl Σ d -> unbox_decl Σ d = unbox_decl Σ' d.
 Proof.
   intros hast ext wf []; cbn.
-  unfold optimize_constant_decl.
+  unfold unbox_constant_decl.
   destruct (EAst.cst_body c) eqn:hc => /= //.
   intros hwf. f_equal. f_equal. f_equal.
-  eapply optimize_extends => //. exact hwf.
+  eapply unbox_extends => //. exact hwf.
   intros _ => //.
 Qed.
 
 From MetaCoq.Erasure Require Import EGenericGlobalMap.
 
 #[local]
-Instance GT : GenTransform := { gen_transform := optimize; gen_transform_inductive_decl := optimize_inductive_decl }.
+Instance GT : GenTransform := { gen_transform := unbox; gen_transform_inductive_decl := unbox_inductive_decl }.
 #[local]
 Instance GTExt efl : has_tApp -> GenTransformExtends efl efl GT.
 Proof.
   intros hasapp Σ t n wfΣ Σ' ext wf wf'.
   unfold gen_transform, GT.
-  eapply optimize_extends; tea.
+  eapply unbox_extends; tea.
 Qed.
 #[local]
 Instance GTWf efl : GenTransformWf efl (switch_no_params efl) GT.
@@ -1322,55 +1292,55 @@ Proof.
   refine {| gen_transform_pre := fun _ _ => has_tApp /\ cstr_as_blocks = false |}; auto.
   - unfold wf_minductive; intros []. cbn. repeat rtoProp. intuition auto.
   - intros Σ n t [? ?] wfΣ wft. unfold gen_transform_env, gen_transform. simpl.
-    eapply optimize_wellformed => //.
+    eapply unbox_wellformed => //.
 Defined.
 
-Lemma optimize_extends' {efl : EEnvFlags} {Σ Σ' : GlobalContextMap.t} :
+Lemma unbox_extends' {efl : EEnvFlags} {Σ Σ' : GlobalContextMap.t} :
   has_tApp ->
   extends Σ Σ' ->
   wf_glob Σ ->
   wf_glob Σ' ->
-  List.map (on_snd (optimize_decl Σ)) Σ.(GlobalContextMap.global_decls) =
-  List.map (on_snd (optimize_decl Σ')) Σ.(GlobalContextMap.global_decls).
+  List.map (on_snd (unbox_decl Σ)) Σ.(GlobalContextMap.global_decls) =
+  List.map (on_snd (unbox_decl Σ')) Σ.(GlobalContextMap.global_decls).
 Proof.
   intros hast ext wf.
   now apply (gen_transform_env_extends' (gt := GTExt efl hast) ext).
 Qed.
 
-Lemma optimize_extends_env {efl : EEnvFlags} {Σ Σ' : GlobalContextMap.t} :
+Lemma unbox_extends_env {efl : EEnvFlags} {Σ Σ' : GlobalContextMap.t} :
   has_tApp ->
   extends Σ Σ' ->
   wf_glob Σ ->
   wf_glob Σ' ->
-  extends (optimize_env Σ) (optimize_env Σ').
+  extends (unbox_env Σ) (unbox_env Σ').
 Proof.
   intros hast ext wf.
   now apply (gen_transform_extends (gt := GTExt efl hast) ext).
 Qed.
 
-Lemma optimize_env_eq (efl := all_env_flags) (Σ : GlobalContextMap.t) : wf_glob Σ -> optimize_env Σ = optimize_env' Σ.(GlobalContextMap.global_decls) Σ.(GlobalContextMap.wf).
+Lemma unbox_env_eq (efl := all_env_flags) (Σ : GlobalContextMap.t) : wf_glob Σ -> unbox_env Σ = unbox_env' Σ.(GlobalContextMap.global_decls) Σ.(GlobalContextMap.wf).
 Proof.
   intros wf.
-  unfold optimize_env.
+  unfold unbox_env.
   destruct Σ; cbn. cbn in wf.
   induction global_decls in map, repr, wf0, wf |- * => //.
   cbn. f_equal.
   destruct a as [kn d]; unfold on_snd; cbn. f_equal. symmetry.
-  eapply optimize_decl_extends => //. cbn. cbn. eapply EExtends.extends_prefix_extends. now exists [(kn, d)]. auto. cbn. now depelim wf.
+  eapply unbox_decl_extends => //. cbn. cbn. eapply EExtends.extends_prefix_extends. now exists [(kn, d)]. auto. cbn. now depelim wf.
   set (Σg' := GlobalContextMap.make global_decls (fresh_globals_cons_inv wf0)).
   erewrite <- (IHglobal_decls (GlobalContextMap.map Σg') (GlobalContextMap.repr Σg')).
   2:now depelim wf.
   set (Σg := {| GlobalContextMap.global_decls := _ :: _ |}).
-  symmetry. eapply (optimize_extends' (Σ := Σg') (Σ' := Σg)) => //.
+  symmetry. eapply (unbox_extends' (Σ := Σg') (Σ' := Σg)) => //.
   cbn. eapply EExtends.extends_prefix_extends => //. now exists [a].
   cbn. now depelim wf.
 Qed.
 
-Lemma optimize_env_wf (efl := all_env_flags) {Σ : GlobalContextMap.t} :
-  wf_glob Σ -> wf_glob (efl := switch_no_params efl) (optimize_env Σ).
+Lemma unbox_env_wf (efl := all_env_flags) {Σ : GlobalContextMap.t} :
+  wf_glob Σ -> wf_glob (efl := switch_no_params efl) (unbox_env Σ).
 Proof.
   intros wf.
-  rewrite (optimize_env_eq _ wf).
+  rewrite (unbox_env_eq _ wf).
   destruct Σ as [Σ map repr fr]; cbn in *.
   induction Σ in map, repr, fr, wf |- *.
   - cbn. constructor.
@@ -1379,111 +1349,111 @@ Proof.
     constructor; eauto.
     eapply (IHΣ (GlobalContextMap.map Σg) (GlobalContextMap.repr Σg)). now depelim wf.
     depelim wf. cbn.
-    rewrite -(optimize_env_eq Σg). now cbn. cbn.
-    now eapply (optimize_decl_wf (Σ:=Σg)).
-    rewrite -(optimize_env_eq Σg). now depelim wf.
-    eapply fresh_global_optimize_env. now depelim fr.
+    rewrite -(unbox_env_eq Σg). now cbn. cbn.
+    now eapply (unbox_decl_wf (Σ:=Σg)).
+    rewrite -(unbox_env_eq Σg). now depelim wf.
+    eapply fresh_global_unbox_env. now depelim fr.
 Qed.
 
-Lemma optimize_program_wf (efl := all_env_flags) (p : eprogram_env) :
+Lemma unbox_program_wf (efl := all_env_flags) (p : eprogram_env) :
   wf_eprogram_env efl p ->
-  wf_eprogram (switch_no_params efl) (optimize_program p).
+  wf_eprogram (switch_no_params efl) (unbox_program p).
 Proof.
   intros []; split => //.
-  eapply (optimize_env_wf H).
-  now eapply optimize_wellformed.
+  eapply (unbox_env_wf H).
+  now eapply unbox_wellformed.
 Qed.
 
-Lemma optimize_expanded {Σ : GlobalContextMap.t} {t} : expanded Σ t -> expanded (optimize_env Σ) (optimize Σ t).
+Lemma unbox_expanded {Σ : GlobalContextMap.t} {t} : expanded Σ t -> expanded (unbox_env Σ) (unbox Σ t).
 Proof.
   induction 1 using expanded_ind.
-  all:try solve[simp_optimize; constructor; eauto; solve_all].
-  - rewrite optimize_mkApps_etaexp. now eapply expanded_isEtaExp.
+  all:try solve[simp_unbox; constructor; eauto; solve_all].
+  - rewrite unbox_mkApps_etaexp. now eapply expanded_isEtaExp.
     eapply expanded_mkApps_expanded => //. solve_all.
-  - simp_optimize; constructor; eauto. solve_all.
-    rewrite -optimize_isLambda //.
-  - rewrite optimize_mkApps // /=.
+  - simp_unbox; constructor; eauto. solve_all.
+    rewrite -unbox_isLambda //.
+  - rewrite unbox_mkApps // /=.
     rewrite (lookup_inductive_pars_spec (proj1 (proj1 H))).
     eapply expanded_tConstruct_app.
-    eapply optimize_declared_constructor; tea.
+    eapply unbox_declared_constructor; tea.
     len. rewrite skipn_length /= /EAst.cstr_arity /=.
     rewrite /EAst.cstr_arity in H0. lia.
     solve_all. eapply All_skipn. solve_all.
 Qed.
 
-Lemma optimize_expanded_irrel {efl : EEnvFlags} {Σ : GlobalContextMap.t} t : wf_glob Σ -> expanded Σ t -> expanded (optimize_env Σ) t.
+Lemma unbox_expanded_irrel {efl : EEnvFlags} {Σ : GlobalContextMap.t} t : wf_glob Σ -> expanded Σ t -> expanded (unbox_env Σ) t.
 Proof.
   intros wf; induction 1 using expanded_ind.
   all:try solve[constructor; eauto; solve_all].
   eapply expanded_tConstruct_app.
   destruct H as [[H ?] ?].
   split => //. split => //. red.
-  red in H. rewrite lookup_env_optimize // /= H //. 1-2:eauto.
+  red in H. rewrite lookup_env_unbox // /= H //. 1-2:eauto.
   cbn. rewrite /EAst.cstr_arity in H0. lia. solve_all.
 Qed.
 
-Lemma optimize_expanded_decl {Σ : GlobalContextMap.t} t : expanded_decl Σ t -> expanded_decl (optimize_env Σ) (optimize_decl Σ t).
+Lemma unbox_expanded_decl {Σ : GlobalContextMap.t} t : expanded_decl Σ t -> expanded_decl (unbox_env Σ) (unbox_decl Σ t).
 Proof.
   destruct t as [[[]]|] => /= //.
   unfold expanded_constant_decl => /=.
-  apply optimize_expanded.
+  apply unbox_expanded.
 Qed.
 
-Lemma optimize_env_expanded (efl := all_env_flags) {Σ : GlobalContextMap.t} :
-  wf_glob Σ -> expanded_global_env Σ -> expanded_global_env (optimize_env Σ).
+Lemma unbox_env_expanded (efl := all_env_flags) {Σ : GlobalContextMap.t} :
+  wf_glob Σ -> expanded_global_env Σ -> expanded_global_env (unbox_env Σ).
 Proof.
   unfold expanded_global_env.
-  intros wf. rewrite optimize_env_eq //.
+  intros wf. rewrite unbox_env_eq //.
   destruct Σ as [Σ map repr wf']; cbn in *.
   intros exp; induction exp in map, repr, wf', wf |- *; cbn.
   - constructor; auto.
   - set (Σ' := GlobalContextMap.make Σ (fresh_globals_cons_inv wf')).
     constructor; auto.
     eapply IHexp. eapply Σ'. now depelim wf. cbn.
-    eapply (optimize_expanded_decl (Σ := Σ')) in H.
-    rewrite -(optimize_env_eq Σ'). cbn. now depelim wf.
+    eapply (unbox_expanded_decl (Σ := Σ')) in H.
+    rewrite -(unbox_env_eq Σ'). cbn. now depelim wf.
     exact H.
 Qed.
 
 Import EProgram.
 
-Lemma optimize_program_expanded (efl := all_env_flags) (p : eprogram_env) :
+Lemma unbox_program_expanded (efl := all_env_flags) (p : eprogram_env) :
   wf_eprogram_env efl p ->
   expanded_eprogram_env_cstrs p ->
-  expanded_eprogram_cstrs (optimize_program p).
+  expanded_eprogram_cstrs (unbox_program p).
 Proof.
   unfold expanded_eprogram_env_cstrs, expanded_eprogram_cstrs.
   move=> [] wfe wft. move/andP => [] etaenv etap.
   apply/andP; split.
-  eapply expanded_global_env_isEtaExp_env, optimize_env_expanded => //.
+  eapply expanded_global_env_isEtaExp_env, unbox_env_expanded => //.
   now eapply isEtaExp_env_expanded_global_env.
-  now eapply expanded_isEtaExp, optimize_expanded, isEtaExp_expanded.
+  now eapply expanded_isEtaExp, unbox_expanded, isEtaExp_expanded.
 Qed.
 
 
-        tConstruct ind n (map optimize args)
-    | tPrim p => tPrim (map_prim optimize p)
+        tConstruct ind n (map unbox args)
+    | tPrim p => tPrim (map_prim unbox p)
     end.
 
-  Lemma optimize_mkApps f l : optimize (mkApps f l) = mkApps (optimize f) (map optimize l).
+  Lemma unbox_mkApps f l : unbox (mkApps f l) = mkApps (unbox f) (map unbox l).
   Proof using Type.
     induction l using rev_ind; simpl; auto.
     now rewrite mkApps_app /= IHl map_app /= mkApps_app /=.
   Qed.
 
-  Lemma map_optimize_repeat_box n : map optimize (repeat tBox n) = repeat tBox n.
+  Lemma map_unbox_repeat_box n : map unbox (repeat tBox n) = repeat tBox n.
   Proof using Type. by rewrite map_repeat. Qed.
 
   (* move to globalenv *)
 
-  Lemma isLambda_optimize t : isLambda t -> isLambda (optimize t).
+  Lemma isLambda_unbox t : isLambda t -> isLambda (unbox t).
   Proof. destruct t => //. Qed.
-  Lemma isBox_optimize t : isBox t -> isBox (optimize t).
+  Lemma isBox_unbox t : isBox t -> isBox (unbox t).
   Proof. destruct t => //. Qed.
 
-  Lemma wf_optimize t k :
+  Lemma wf_unbox t k :
     wf_glob Σ ->
-    wellformed Σ k t -> wellformed Σ k (optimize t).
+    wellformed Σ k t -> wellformed Σ k (unbox t).
   Proof using Type.
     intros wfΣ.
     induction t in k |- * using EInduction.term_forall_list_ind; simpl; auto;
@@ -1503,15 +1473,15 @@ Qed.
       rewrite IHt //=; len. apply Nat.ltb_lt.
       lia.
     - len. rtoProp; solve_all. solve_all.
-      now eapply isLambda_optimize. solve_all.
+      now eapply isLambda_unbox. solve_all.
     - len. rtoProp; repeat solve_all.
     - rewrite test_prim_map. rtoProp; intuition eauto; solve_all.
   Qed.
 
-  Lemma optimize_csubst {a k b} n :
+  Lemma unbox_csubst {a k b} n :
     wf_glob Σ ->
     wellformed Σ (k + n) b ->
-    optimize (ECSubst.csubst a k b) = ECSubst.csubst (optimize a) k (optimize b).
+    unbox (ECSubst.csubst a k b) = ECSubst.csubst (unbox a) k (unbox b).
   Proof using Type.
     intros wfΣ.
     induction b in k |- * using EInduction.term_forall_list_ind; simpl; auto;
@@ -1539,33 +1509,33 @@ Qed.
       eapply a0. now rewrite -Nat.add_assoc.
   Qed.
 
-  Lemma optimize_substl s t :
+  Lemma unbox_substl s t :
     wf_glob Σ ->
     forallb (wellformed Σ 0) s ->
     wellformed Σ #|s| t ->
-    optimize (substl s t) = substl (map optimize s) (optimize t).
+    unbox (substl s t) = substl (map unbox s) (unbox t).
   Proof using Type.
     intros wfΣ. induction s in t |- *; simpl; auto.
     move/andP => [] cla cls wft.
     rewrite IHs //. eapply wellformed_csubst => //.
-    f_equal. rewrite (optimize_csubst (S #|s|)) //.
+    f_equal. rewrite (unbox_csubst (S #|s|)) //.
   Qed.
 
-  Lemma optimize_iota_red pars args br :
+  Lemma unbox_iota_red pars args br :
     wf_glob Σ ->
     forallb (wellformed Σ 0) args ->
     wellformed Σ #|skipn pars args| br.2 ->
-    optimize (EGlobalEnv.iota_red pars args br) = EGlobalEnv.iota_red pars (map optimize args) (on_snd optimize br).
+    unbox (EGlobalEnv.iota_red pars args br) = EGlobalEnv.iota_red pars (map unbox args) (on_snd unbox br).
   Proof using Type.
     intros wfΣ wfa wfbr.
     unfold EGlobalEnv.iota_red.
-    rewrite optimize_substl //.
+    rewrite unbox_substl //.
     rewrite forallb_rev forallb_skipn //.
     now rewrite List.rev_length.
     now rewrite map_rev map_skipn.
   Qed.
 
-  Lemma optimize_fix_subst mfix : EGlobalEnv.fix_subst (map (map_def optimize) mfix) = map optimize (EGlobalEnv.fix_subst mfix).
+  Lemma unbox_fix_subst mfix : EGlobalEnv.fix_subst (map (map_def unbox) mfix) = map unbox (EGlobalEnv.fix_subst mfix).
   Proof using Type.
     unfold EGlobalEnv.fix_subst.
     rewrite map_length.
@@ -1574,7 +1544,7 @@ Qed.
     f_equal; auto.
   Qed.
 
-  Lemma optimize_cofix_subst mfix : EGlobalEnv.cofix_subst (map (map_def optimize) mfix) = map optimize (EGlobalEnv.cofix_subst mfix).
+  Lemma unbox_cofix_subst mfix : EGlobalEnv.cofix_subst (map (map_def unbox) mfix) = map unbox (EGlobalEnv.cofix_subst mfix).
   Proof using Type.
     unfold EGlobalEnv.cofix_subst.
     rewrite map_length.
@@ -1583,11 +1553,11 @@ Qed.
     f_equal; auto.
   Qed.
 
-  Lemma optimize_cunfold_fix mfix idx n f :
+  Lemma unbox_cunfold_fix mfix idx n f :
     wf_glob Σ ->
     wellformed Σ 0 (tFix mfix idx) ->
     cunfold_fix mfix idx = Some (n, f) ->
-    cunfold_fix (map (map_def optimize) mfix) idx = Some (n, optimize f).
+    cunfold_fix (map (map_def unbox) mfix) idx = Some (n, unbox f).
   Proof using Type.
     intros wfΣ hfix.
     unfold cunfold_fix.
@@ -1595,17 +1565,17 @@ Qed.
     cbn in hfix. move/andP: hfix => [] hlam /andP[] hidx hfix.
     destruct nth_error eqn:hnth => //.
     intros [= <- <-] => /=. f_equal.
-    rewrite optimize_substl //. eapply wellformed_fix_subst => //.
+    rewrite unbox_substl //. eapply wellformed_fix_subst => //.
     rewrite fix_subst_length.
     eapply nth_error_forallb in hfix; tea. now rewrite Nat.add_0_r in hfix.
-    now rewrite optimize_fix_subst.
+    now rewrite unbox_fix_subst.
   Qed.
 
-  Lemma optimize_cunfold_cofix mfix idx n f :
+  Lemma unbox_cunfold_cofix mfix idx n f :
     wf_glob Σ ->
     wellformed Σ 0 (tCoFix mfix idx) ->
     cunfold_cofix mfix idx = Some (n, f) ->
-    cunfold_cofix (map (map_def optimize) mfix) idx = Some (n, optimize f).
+    cunfold_cofix (map (map_def unbox) mfix) idx = Some (n, unbox f).
   Proof using Type.
     intros wfΣ hfix.
     unfold cunfold_cofix.
@@ -1613,34 +1583,34 @@ Qed.
     cbn in hfix. move/andP: hfix => [] hidx hfix.
     destruct nth_error eqn:hnth => //.
     intros [= <- <-] => /=. f_equal.
-    rewrite optimize_substl //. eapply wellformed_cofix_subst => //.
+    rewrite unbox_substl //. eapply wellformed_cofix_subst => //.
     rewrite cofix_subst_length.
     eapply nth_error_forallb in hfix; tea. now rewrite Nat.add_0_r in hfix.
-    now rewrite optimize_cofix_subst.
+    now rewrite unbox_cofix_subst.
   Qed.
 
-End optimize.
+End unbox.
 
-Definition optimize_constant_decl Σ cb :=
-  {| cst_body := option_map (optimize Σ) cb.(cst_body) |}.
+Definition unbox_constant_decl Σ cb :=
+  {| cst_body := option_map (unbox Σ) cb.(cst_body) |}.
 
-Definition optimize_decl Σ d :=
+Definition unbox_decl Σ d :=
   match d with
-  | ConstantDecl cb => ConstantDecl (optimize_constant_decl Σ cb)
+  | ConstantDecl cb => ConstantDecl (unbox_constant_decl Σ cb)
   | InductiveDecl idecl => InductiveDecl idecl
   end.
 
-Definition optimize_env Σ :=
-  map (on_snd (optimize_decl Σ)) Σ.(GlobalContextMap.global_decls).
+Definition unbox_env Σ :=
+  map (on_snd (unbox_decl Σ)) Σ.(GlobalContextMap.global_decls).
 
 Import EnvMap.
 
-Program Fixpoint optimize_env' Σ : EnvMap.fresh_globals Σ -> global_context :=
+Program Fixpoint unbox_env' Σ : EnvMap.fresh_globals Σ -> global_context :=
   match Σ with
   | [] => fun _ => []
   | hd :: tl => fun HΣ =>
     let Σg := GlobalContextMap.make tl (fresh_globals_cons_inv HΣ) in
-    on_snd (optimize_decl Σg) hd :: optimize_env' tl (fresh_globals_cons_inv HΣ)
+    on_snd (unbox_decl Σg) hd :: unbox_env' tl (fresh_globals_cons_inv HΣ)
   end.
 
 Import EGlobalEnv EExtends.
@@ -1656,10 +1626,10 @@ Proof.
   rewrite (extends_lookup_constructor wf ext _ _ _ hl) //.
 Qed.
 
-Lemma wellformed_optimize_extends {wfl: EEnvFlags} {Σ : GlobalContextMap.t} t :
+Lemma wellformed_unbox_extends {wfl: EEnvFlags} {Σ : GlobalContextMap.t} t :
   forall n, EWellformed.wellformed Σ n t ->
   forall {Σ' : GlobalContextMap.t}, extends Σ Σ' -> wf_glob Σ' ->
-  optimize Σ t = optimize Σ' t.
+  unbox Σ t = unbox Σ' t.
 Proof.
   induction t using EInduction.term_forall_list_ind; cbn -[lookup_constant lookup_inductive
     GlobalContextMap.lookup_projection]; intros => //.
@@ -1672,23 +1642,23 @@ Proof.
     now cbn in H3.
 Qed.
 
-Lemma wellformed_optimize_decl_extends {wfl: EEnvFlags} {Σ : GlobalContextMap.t} t :
+Lemma wellformed_unbox_decl_extends {wfl: EEnvFlags} {Σ : GlobalContextMap.t} t :
   wf_global_decl Σ t ->
   forall {Σ' : GlobalContextMap.t}, extends Σ Σ' -> wf_glob Σ' ->
-  optimize_decl Σ t = optimize_decl Σ' t.
+  unbox_decl Σ t = unbox_decl Σ' t.
 Proof.
   destruct t => /= //.
-  intros wf Σ' ext wf'. f_equal. unfold optimize_constant_decl. f_equal.
+  intros wf Σ' ext wf'. f_equal. unfold unbox_constant_decl. f_equal.
   destruct (cst_body c) => /= //. f_equal.
-  now eapply wellformed_optimize_extends.
+  now eapply wellformed_unbox_extends.
 Qed.
 
-Lemma lookup_env_optimize_env_Some {efl : EEnvFlags} {Σ : GlobalContextMap.t} kn d :
+Lemma lookup_env_unbox_env_Some {efl : EEnvFlags} {Σ : GlobalContextMap.t} kn d :
   wf_glob Σ ->
   GlobalContextMap.lookup_env Σ kn = Some d ->
   ∑ Σ' : GlobalContextMap.t,
     [× extends_prefix Σ' Σ, wf_global_decl Σ' d &
-      lookup_env (optimize_env Σ) kn = Some (optimize_decl Σ' d)].
+      lookup_env (unbox_env Σ) kn = Some (unbox_decl Σ' d)].
 Proof.
   rewrite GlobalContextMap.lookup_env_spec.
   destruct Σ as [Σ map repr wf].
@@ -1699,7 +1669,7 @@ Proof.
     exists (GlobalContextMap.make Σ (fresh_globals_cons_inv wf)). split.
     now eexists [_].
     cbn. now depelim wfg.
-    f_equal. symmetry. eapply wellformed_optimize_decl_extends. cbn. now depelim wfg.
+    f_equal. symmetry. eapply wellformed_unbox_decl_extends. cbn. now depelim wfg.
     eapply extends_prefix_extends.
     cbn. now exists [a]. now cbn. now cbn.
   - intros _.
@@ -1713,7 +1683,7 @@ Proof.
     * rewrite -hl'. f_equal.
       clear -wfg.
       eapply map_ext_in => kn hin. unfold on_snd. f_equal.
-      symmetry. eapply wellformed_optimize_decl_extends => //. cbn.
+      symmetry. eapply wellformed_unbox_decl_extends => //. cbn.
       eapply lookup_env_In in hin. 2:now depelim wfg.
       depelim wfg. eapply lookup_env_wellformed; tea.
       eapply extends_prefix_extends.
@@ -1726,60 +1696,60 @@ Proof.
   case: eqb_spec => //.
 Qed.
 
-Lemma lookup_env_optimize_env_None {efl : EEnvFlags} {Σ : GlobalContextMap.t} kn :
+Lemma lookup_env_unbox_env_None {efl : EEnvFlags} {Σ : GlobalContextMap.t} kn :
   GlobalContextMap.lookup_env Σ kn = None ->
-  lookup_env (optimize_env Σ) kn = None.
+  lookup_env (unbox_env Σ) kn = None.
 Proof.
   rewrite GlobalContextMap.lookup_env_spec.
   destruct Σ as [Σ map repr wf].
   cbn. intros hl. rewrite lookup_env_map_snd hl //.
 Qed.
 
-Lemma lookup_env_optimize {efl : EEnvFlags} {Σ : GlobalContextMap.t} kn :
+Lemma lookup_env_unbox {efl : EEnvFlags} {Σ : GlobalContextMap.t} kn :
   wf_glob Σ ->
-  lookup_env (optimize_env Σ) kn = option_map (optimize_decl Σ) (lookup_env Σ kn).
+  lookup_env (unbox_env Σ) kn = option_map (unbox_decl Σ) (lookup_env Σ kn).
 Proof.
   intros wf.
   rewrite -GlobalContextMap.lookup_env_spec.
   destruct (GlobalContextMap.lookup_env Σ kn) eqn:hl.
-  - eapply lookup_env_optimize_env_Some in hl as [Σ' [ext wf' hl']] => /=.
+  - eapply lookup_env_unbox_env_Some in hl as [Σ' [ext wf' hl']] => /=.
     rewrite hl'. f_equal.
-    eapply wellformed_optimize_decl_extends; eauto.
+    eapply wellformed_unbox_decl_extends; eauto.
     now eapply extends_prefix_extends. auto.
 
-  - cbn. now eapply lookup_env_optimize_env_None in hl.
+  - cbn. now eapply lookup_env_unbox_env_None in hl.
 Qed.
 
-Lemma is_propositional_optimize {efl : EEnvFlags} {Σ : GlobalContextMap.t} ind :
+Lemma is_propositional_unbox {efl : EEnvFlags} {Σ : GlobalContextMap.t} ind :
   wf_glob Σ ->
-  inductive_isprop_and_pars Σ ind = inductive_isprop_and_pars (optimize_env Σ) ind.
+  inductive_isprop_and_pars Σ ind = inductive_isprop_and_pars (unbox_env Σ) ind.
 Proof.
   rewrite /inductive_isprop_and_pars => wf.
   rewrite /lookup_inductive /lookup_minductive.
-  rewrite (lookup_env_optimize (inductive_mind ind) wf).
+  rewrite (lookup_env_unbox (inductive_mind ind) wf).
   rewrite /GlobalContextMap.inductive_isprop_and_pars /GlobalContextMap.lookup_inductive
     /GlobalContextMap.lookup_minductive.
   destruct lookup_env as [[decl|]|] => //.
 Qed.
 
-Lemma lookup_inductive_pars_optimize {efl : EEnvFlags} {Σ : GlobalContextMap.t} ind :
+Lemma lookup_inductive_pars_unbox {efl : EEnvFlags} {Σ : GlobalContextMap.t} ind :
   wf_glob Σ ->
-  EGlobalEnv.lookup_inductive_pars Σ ind = EGlobalEnv.lookup_inductive_pars (optimize_env Σ) ind.
+  EGlobalEnv.lookup_inductive_pars Σ ind = EGlobalEnv.lookup_inductive_pars (unbox_env Σ) ind.
 Proof.
   rewrite /lookup_inductive_pars => wf.
   rewrite /lookup_inductive /lookup_minductive.
-  rewrite (lookup_env_optimize ind wf).
+  rewrite (lookup_env_unbox ind wf).
   rewrite /GlobalContextMap.lookup_inductive /GlobalContextMap.lookup_minductive.
   destruct lookup_env as [[decl|]|] => //.
 Qed.
 
-Lemma is_propositional_cstr_optimize {efl : EEnvFlags} {Σ : GlobalContextMap.t} ind c :
+Lemma is_propositional_cstr_unbox {efl : EEnvFlags} {Σ : GlobalContextMap.t} ind c :
   wf_glob Σ ->
-  constructor_isprop_pars_decl Σ ind c = constructor_isprop_pars_decl (optimize_env Σ) ind c.
+  constructor_isprop_pars_decl Σ ind c = constructor_isprop_pars_decl (unbox_env Σ) ind c.
 Proof.
   rewrite /constructor_isprop_pars_decl => wf.
   rewrite /lookup_constructor /lookup_inductive /lookup_minductive.
-  rewrite (lookup_env_optimize (inductive_mind ind) wf).
+  rewrite (lookup_env_unbox (inductive_mind ind) wf).
   rewrite /GlobalContextMap.inductive_isprop_and_pars /GlobalContextMap.lookup_inductive
     /GlobalContextMap.lookup_minductive.
   destruct lookup_env as [[decl|]|] => //.
@@ -1809,21 +1779,21 @@ Proof.
   - rewrite mkApps_app /=. now destruct l => /= //; rewrite andb_false_r.
 Qed.
 
-Lemma lookup_constructor_optimize {efl : EEnvFlags} {Σ : GlobalContextMap.t} {ind c} :
+Lemma lookup_constructor_unbox {efl : EEnvFlags} {Σ : GlobalContextMap.t} {ind c} :
   wf_glob Σ ->
-  lookup_constructor Σ ind c = lookup_constructor (optimize_env Σ) ind c.
+  lookup_constructor Σ ind c = lookup_constructor (unbox_env Σ) ind c.
 Proof.
   intros wfΣ. rewrite /lookup_constructor /lookup_inductive /lookup_minductive.
-  rewrite lookup_env_optimize // /=. destruct lookup_env => // /=.
+  rewrite lookup_env_unbox // /=. destruct lookup_env => // /=.
   destruct g => //.
 Qed.
 
-Lemma lookup_projection_optimize {efl : EEnvFlags} {Σ : GlobalContextMap.t} {p} :
+Lemma lookup_projection_unbox {efl : EEnvFlags} {Σ : GlobalContextMap.t} {p} :
   wf_glob Σ ->
-  lookup_projection Σ p = lookup_projection (optimize_env Σ) p.
+  lookup_projection Σ p = lookup_projection (unbox_env Σ) p.
 Proof.
   intros wfΣ. rewrite /lookup_projection.
-  rewrite -lookup_constructor_optimize //.
+  rewrite -lookup_constructor_unbox //.
 Qed.
 
 Lemma constructor_isprop_pars_decl_inductive {Σ ind c} {prop pars cdecl} :
@@ -1867,11 +1837,11 @@ Proof.
 Qed.
 
 
-Lemma optimize_correct {fl} {wcon : with_constructor_as_block = false} { Σ : GlobalContextMap.t} t v :
+Lemma unbox_correct {fl} {wcon : with_constructor_as_block = false} { Σ : GlobalContextMap.t} t v :
   wf_glob Σ ->
   @eval fl Σ t v ->
   wellformed Σ 0 t ->
-  @eval fl (optimize_env Σ) (optimize Σ t) (optimize Σ v).
+  @eval fl (unbox_env Σ) (unbox Σ t) (unbox Σ v).
 Proof.
   intros wfΣ ev.
   induction ev; simpl in *.
@@ -1881,24 +1851,24 @@ Proof.
     eapply eval_wellformed in ev2; tea => //.
     eapply eval_wellformed in ev1; tea => //.
     econstructor; eauto.
-    rewrite -(optimize_csubst _ 1) //.
+    rewrite -(unbox_csubst _ 1) //.
     apply IHev3. eapply wellformed_csubst => //.
 
   - move/andP => [] clb0 clb1.
     intuition auto.
     eapply eval_wellformed in ev1; tea => //.
     forward IHev2 by eapply wellformed_csubst => //.
-    econstructor; eauto. rewrite -(optimize_csubst _ 1) //.
+    econstructor; eauto. rewrite -(unbox_csubst _ 1) //.
 
-  - move/andP => [] /andP[] hl wfd wfbrs. rewrite optimize_mkApps in IHev1.
+  - move/andP => [] /andP[] hl wfd wfbrs. rewrite unbox_mkApps in IHev1.
     eapply eval_wellformed in ev1 => //.
     move/wf_mkApps: ev1 => [] wfc' wfargs.
     eapply nth_error_forallb in wfbrs; tea.
     rewrite Nat.add_0_r in wfbrs.
     forward IHev2. eapply wellformed_iota_red; tea => //.
-    rewrite optimize_iota_red in IHev2 => //. now rewrite e4.
+    rewrite unbox_iota_red in IHev2 => //. now rewrite e4.
     econstructor; eauto.
-    rewrite -is_propositional_cstr_optimize //. tea.
+    rewrite -is_propositional_cstr_unbox //. tea.
     rewrite nth_error_map e2 //. len. len.
 
   - congruence.
@@ -1907,22 +1877,22 @@ Proof.
     forward IHev2. eapply wellformed_substl; tea => //.
     rewrite forallb_repeat //. len.
     rewrite e1 /= Nat.add_0_r in wfbrs. now move/andP: wfbrs.
-    rewrite optimize_substl in IHev2 => //.
+    rewrite unbox_substl in IHev2 => //.
     rewrite forallb_repeat //. len.
     rewrite e1 /= Nat.add_0_r in wfbrs. now move/andP: wfbrs.
     eapply eval_iota_sing => //; eauto.
-    rewrite -is_propositional_optimize //.
+    rewrite -is_propositional_unbox //.
     rewrite e1 //. simpl.
     rewrite map_repeat in IHev2 => //.
 
-  - move/andP => [] clf cla. rewrite optimize_mkApps in IHev1.
+  - move/andP => [] clf cla. rewrite unbox_mkApps in IHev1.
     simpl in *.
     eapply eval_wellformed in ev1 => //.
     move/wf_mkApps: ev1 => [] wff wfargs.
     eapply eval_fix; eauto.
     rewrite map_length.
-    eapply optimize_cunfold_fix; tea.
-    rewrite optimize_mkApps in IHev3. apply IHev3.
+    eapply unbox_cunfold_fix; tea.
+    rewrite unbox_mkApps in IHev3. apply IHev3.
     rewrite wellformed_mkApps // wfargs.
     eapply eval_wellformed in ev2; tas => //. rewrite ev2 /= !andb_true_r.
     eapply wellformed_cunfold_fix; tea.
@@ -1931,16 +1901,16 @@ Proof.
     eapply eval_wellformed in ev1 => //.
     move/wf_mkApps: ev1 => [] clfix clargs.
     eapply eval_wellformed in ev2; tas => //.
-    rewrite optimize_mkApps in IHev1 |- *.
+    rewrite unbox_mkApps in IHev1 |- *.
     simpl in *. eapply eval_fix_value. auto. auto. auto.
-    eapply optimize_cunfold_fix; eauto.
+    eapply unbox_cunfold_fix; eauto.
     now rewrite map_length.
 
   - move/andP => [] clf cla.
     eapply eval_wellformed in ev1 => //.
     eapply eval_wellformed in ev2; tas => //.
     simpl in *. eapply eval_fix'. auto. auto.
-    eapply optimize_cunfold_fix; eauto.
+    eapply unbox_cunfold_fix; eauto.
     eapply IHev2; tea. eapply IHev3.
     apply/andP; split => //.
     eapply wellformed_cunfold_fix; tea. now cbn.
@@ -1951,9 +1921,9 @@ Proof.
     forward IHev2.
     rewrite hl wellformed_mkApps // /= wfargs clbrs !andb_true_r.
     eapply wellformed_cunfold_cofix; tea => //.
-    rewrite !optimize_mkApps /= in IHev1, IHev2.
+    rewrite !unbox_mkApps /= in IHev1, IHev2.
     eapply eval_cofix_case. tea.
-    eapply optimize_cunfold_cofix; tea.
+    eapply unbox_cunfold_cofix; tea.
     exact IHev2.
 
   - move/andP => [] hl hd.
@@ -1964,13 +1934,13 @@ Proof.
     forward IHev2.
     { rewrite /= wellformed_mkApps // wfargs andb_true_r.
       eapply wellformed_cunfold_cofix; tea. }
-    rewrite optimize_mkApps /= in IHev1.
+    rewrite unbox_mkApps /= in IHev1.
     eapply eval_cofix_case. eauto.
-    eapply optimize_cunfold_cofix; tea.
-    rewrite optimize_mkApps in IHev2 => //.
+    eapply unbox_cunfold_cofix; tea.
+    rewrite unbox_mkApps in IHev2 => //.
 
   - rewrite /declared_constant in isdecl.
-    move: (lookup_env_optimize c wfΣ).
+    move: (lookup_env_unbox c wfΣ).
     rewrite isdecl /= //.
     intros hl.
     econstructor; tea. cbn. rewrite e //.
@@ -1987,15 +1957,15 @@ Proof.
     rewrite (constructor_isprop_pars_decl_constructor H) in e1. noconf e1.
     forward IHev1 by auto.
     forward IHev2. eapply nth_error_forallb in wfargs; tea.
-    rewrite optimize_mkApps /= in IHev1.
+    rewrite unbox_mkApps /= in IHev1.
     eapply eval_iota; tea.
-    rewrite /constructor_isprop_pars_decl -lookup_constructor_optimize // H //= //.
+    rewrite /constructor_isprop_pars_decl -lookup_constructor_unbox // H //= //.
     rewrite H0 H1; reflexivity. cbn. reflexivity. len. len.
     rewrite skipn_length. lia.
     unfold iota_red. cbn.
-    rewrite (substl_rel _ _ (optimize Σ a)) => //.
+    rewrite (substl_rel _ _ (unbox Σ a)) => //.
     { eapply nth_error_forallb in wfargs; tea.
-      eapply wf_optimize in wfargs => //.
+      eapply wf_unbox in wfargs => //.
       now eapply wellformed_closed in wfargs. }
     pose proof (wellformed_projection_args wfΣ hl'). cbn in H1.
     rewrite nth_error_rev. len. rewrite skipn_length. lia.
@@ -2004,7 +1974,7 @@ Proof.
     rewrite e2 -H1.
     assert((ind_npars mdecl + cstr_nargs cdecl - ind_npars mdecl) = cstr_nargs cdecl) by lia.
     rewrite H3.
-    eapply (f_equal (option_map (optimize Σ))) in e3.
+    eapply (f_equal (option_map (unbox Σ))) in e3.
     cbn in e3. rewrite -e3. f_equal. f_equal. lia.
 
   - congruence.
@@ -2018,7 +1988,7 @@ Proof.
     rewrite (lookup_constructor_lookup_inductive H) /=.
     intros [= eq <-].
     eapply eval_iota_sing => //; eauto.
-    rewrite -is_propositional_optimize // /inductive_isprop_and_pars
+    rewrite -is_propositional_unbox // /inductive_isprop_and_pars
       (lookup_constructor_lookup_inductive H) //=. congruence.
     have lenarg := wellformed_projection_args wfΣ hl'.
     rewrite (substl_rel _ _ tBox) => //.
@@ -2026,10 +1996,10 @@ Proof.
     now constructor.
 
   - move/andP=> [] clf cla.
-    rewrite optimize_mkApps.
+    rewrite unbox_mkApps.
     eapply eval_construct; tea.
-    rewrite -lookup_constructor_optimize //. exact e0.
-    rewrite optimize_mkApps in IHev1. now eapply IHev1.
+    rewrite -lookup_constructor_unbox //. exact e0.
+    rewrite unbox_mkApps in IHev1. now eapply IHev1.
     now len.
     now eapply IHev2.
 
@@ -2041,18 +2011,18 @@ Proof.
     eapply eval_to_value in ev1.
     destruct ev1; simpl in *; eauto.
     * depelim a0.
-      + destruct t => //; rewrite optimize_mkApps /=.
+      + destruct t => //; rewrite unbox_mkApps /=.
       + now rewrite /= !orb_false_r orb_true_r in i.
     * destruct with_guarded_fix.
       + move: i.
         rewrite !negb_or.
-        rewrite optimize_mkApps !isFixApp_mkApps !isConstructApp_mkApps !isPrimApp_mkApps.
+        rewrite unbox_mkApps !isFixApp_mkApps !isConstructApp_mkApps !isPrimApp_mkApps.
         destruct args using rev_case => // /=. rewrite map_app !mkApps_app /= //.
         rewrite !andb_true_r.
         rtoProp; intuition auto;  destruct v => /= //.
       + move: i.
         rewrite !negb_or.
-        rewrite optimize_mkApps !isConstructApp_mkApps !isPrimApp_mkApps.
+        rewrite unbox_mkApps !isConstructApp_mkApps !isPrimApp_mkApps.
         destruct args using rev_case => // /=. rewrite map_app !mkApps_app /= //.
         destruct v => /= //.
   - intros; rtoProp; intuition eauto.
@@ -2063,18 +2033,18 @@ Proof.
     primProp; depelim H0; intuition eauto.
   - destruct t => //.
     all:constructor; eauto.
-    cbn [atom optimize] in i |- *.
-    rewrite -lookup_constructor_optimize //.
+    cbn [atom unbox] in i |- *.
+    rewrite -lookup_constructor_unbox //.
     destruct args; cbn in *; eauto.
 Qed.
 
 From MetaCoq.Erasure Require Import EEtaExpanded.
 
-Lemma optimize_expanded {Σ : GlobalContextMap.t} t : expanded Σ t -> expanded Σ (optimize Σ t).
+Lemma unbox_expanded {Σ : GlobalContextMap.t} t : expanded Σ t -> expanded Σ (unbox Σ t).
 Proof.
   induction 1 using expanded_ind.
   all:try solve[constructor; eauto; solve_all].
-  all:rewrite ?optimize_mkApps.
+  all:rewrite ?unbox_mkApps.
   - eapply expanded_mkApps_expanded => //. solve_all.
   - cbn -[GlobalContextMap.inductive_isprop_and_pars].
     rewrite GlobalContextMap.lookup_projection_spec.
@@ -2083,39 +2053,39 @@ Proof.
     destruct proj as [[ind npars] arg].
     econstructor; eauto. repeat constructor.
   - cbn. eapply expanded_tFix. solve_all.
-    rewrite isLambda_optimize //.
+    rewrite isLambda_unbox //.
   - eapply expanded_tConstruct_app; tea.
     now len. solve_all.
 Qed.
 
-Lemma optimize_expanded_irrel {efl : EEnvFlags} {Σ : GlobalContextMap.t} t : wf_glob Σ -> expanded Σ t -> expanded (optimize_env Σ) t.
+Lemma unbox_expanded_irrel {efl : EEnvFlags} {Σ : GlobalContextMap.t} t : wf_glob Σ -> expanded Σ t -> expanded (unbox_env Σ) t.
 Proof.
   intros wf; induction 1 using expanded_ind.
   all:try solve[constructor; eauto; solve_all].
   eapply expanded_tConstruct_app.
   destruct H as [[H ?] ?].
   split => //. split => //. red.
-  red in H. rewrite lookup_env_optimize // /= H //. 1-2:eauto. auto. solve_all.
+  red in H. rewrite lookup_env_unbox // /= H //. 1-2:eauto. auto. solve_all.
 Qed.
 
-Lemma optimize_expanded_decl {Σ : GlobalContextMap.t} t : expanded_decl Σ t -> expanded_decl Σ (optimize_decl Σ t).
+Lemma unbox_expanded_decl {Σ : GlobalContextMap.t} t : expanded_decl Σ t -> expanded_decl Σ (unbox_decl Σ t).
 Proof.
   destruct t as [[[]]|] => /= //.
   unfold expanded_constant_decl => /=.
-  apply optimize_expanded.
+  apply unbox_expanded.
 Qed.
 
-Lemma optimize_expanded_decl_irrel {efl : EEnvFlags} {Σ : GlobalContextMap.t} t : wf_glob Σ -> expanded_decl Σ t -> expanded_decl (optimize_env Σ) t.
+Lemma unbox_expanded_decl_irrel {efl : EEnvFlags} {Σ : GlobalContextMap.t} t : wf_glob Σ -> expanded_decl Σ t -> expanded_decl (unbox_env Σ) t.
 Proof.
   destruct t as [[[]]|] => /= //.
   unfold expanded_constant_decl => /=.
-  apply optimize_expanded_irrel.
+  apply unbox_expanded_irrel.
 Qed.
 
-Lemma optimize_wellformed_term {efl : EEnvFlags} {Σ : GlobalContextMap.t} n t :
+Lemma unbox_wellformed_term {efl : EEnvFlags} {Σ : GlobalContextMap.t} n t :
   has_tBox -> has_tRel ->
   wf_glob Σ -> EWellformed.wellformed Σ n t ->
-  EWellformed.wellformed (efl := disable_projections_env_flag efl) Σ n (optimize Σ t).
+  EWellformed.wellformed (efl := disable_projections_env_flag efl) Σ n (unbox Σ t).
 Proof.
   intros hbox hrel wfΣ.
   induction t in n |- * using EInduction.term_forall_list_ind => //.
@@ -2132,50 +2102,50 @@ Proof.
     rewrite hrel IHt //= andb_true_r.
     have hargs' := wellformed_projection_args wfΣ hl'.
     apply Nat.ltb_lt. len.
-  - cbn. unfold wf_fix; rtoProp; intuition auto; solve_all. now eapply isLambda_optimize.
+  - cbn. unfold wf_fix; rtoProp; intuition auto; solve_all. now eapply isLambda_unbox.
   - cbn. unfold wf_fix; rtoProp; intuition auto; solve_all.
   - cbn. rtoProp; intuition eauto; solve_all_k 6.
 Qed.
 
 Import EWellformed.
 
-Lemma optimize_wellformed_irrel {efl : EEnvFlags} {Σ : GlobalContextMap.t} t :
+Lemma unbox_wellformed_irrel {efl : EEnvFlags} {Σ : GlobalContextMap.t} t :
   wf_glob Σ ->
   forall n, wellformed (efl := disable_projections_env_flag efl) Σ n t ->
-  wellformed (efl := disable_projections_env_flag efl) (optimize_env Σ) n t.
+  wellformed (efl := disable_projections_env_flag efl) (unbox_env Σ) n t.
 Proof.
   intros wfΣ. induction t using EInduction.term_forall_list_ind; cbn => //.
   all:try solve [intros; unfold wf_fix_gen in *; rtoProp; intuition eauto; solve_all].
-  - rewrite lookup_env_optimize //.
+  - rewrite lookup_env_unbox //.
     destruct lookup_env eqn:hl => // /=.
     destruct g eqn:hg => /= //.
     repeat (rtoProp; intuition auto).
     destruct has_axioms => //. cbn in *.
     destruct (cst_body c) => //.
-  - rewrite lookup_env_optimize //.
+  - rewrite lookup_env_unbox //.
     destruct lookup_env eqn:hl => // /=; intros; rtoProp; eauto.
     destruct g eqn:hg => /= //; intros; rtoProp; eauto.
     repeat split; eauto. destruct cstr_as_blocks; rtoProp; repeat split; eauto. solve_all.
-  - rewrite lookup_env_optimize //.
+  - rewrite lookup_env_unbox //.
     destruct lookup_env eqn:hl => // /=.
     destruct g eqn:hg => /= //. subst g.
     destruct nth_error => /= //.
     intros; rtoProp; intuition auto; solve_all.
 Qed.
 
-Lemma optimize_wellformed {efl : EEnvFlags} {Σ : GlobalContextMap.t} n t :
+Lemma unbox_wellformed {efl : EEnvFlags} {Σ : GlobalContextMap.t} n t :
   has_tBox -> has_tRel ->
   wf_glob Σ -> EWellformed.wellformed Σ n t ->
-  EWellformed.wellformed (efl := disable_projections_env_flag efl) (optimize_env Σ) n (optimize Σ t).
+  EWellformed.wellformed (efl := disable_projections_env_flag efl) (unbox_env Σ) n (unbox Σ t).
 Proof.
-  intros. apply optimize_wellformed_irrel => //.
-  now apply optimize_wellformed_term.
+  intros. apply unbox_wellformed_irrel => //.
+  now apply unbox_wellformed_term.
 Qed.
 
 From MetaCoq.Erasure Require Import EGenericGlobalMap.
 
 #[local]
-Instance GT : GenTransform := { gen_transform := optimize; gen_transform_inductive_decl := id }.
+Instance GT : GenTransform := { gen_transform := unbox; gen_transform_inductive_decl := id }.
 #[local]
 Instance GTID : GenTransformId GT.
 Proof.
@@ -2186,47 +2156,47 @@ Instance GTExt efl : GenTransformExtends efl (disable_projections_env_flag efl) 
 Proof.
   intros Σ t n wfΣ Σ' ext wf wf'.
   unfold gen_transform, GT.
-  eapply wellformed_optimize_extends; tea.
+  eapply wellformed_unbox_extends; tea.
 Qed.
 #[local]
 Instance GTWf efl : GenTransformWf efl (disable_projections_env_flag efl) GT.
 Proof.
   refine {| gen_transform_pre := fun _ _ => has_tBox /\ has_tRel |}; auto.
   intros Σ n t [] wfΣ wft.
-  now apply optimize_wellformed.
+  now apply unbox_wellformed.
 Defined.
 
-Lemma optimize_extends_env {efl : EEnvFlags} {Σ Σ' : GlobalContextMap.t} :
+Lemma unbox_extends_env {efl : EEnvFlags} {Σ Σ' : GlobalContextMap.t} :
   has_tApp ->
   extends Σ Σ' ->
   wf_glob Σ ->
   wf_glob Σ' ->
-  extends (optimize_env Σ) (optimize_env Σ').
+  extends (unbox_env Σ) (unbox_env Σ').
 Proof.
   intros hast ext wf.
   now apply (gen_transform_extends (gt := GTExt efl) ext).
 Qed.
 
-Lemma optimize_env_eq {efl : EEnvFlags} (Σ : GlobalContextMap.t) : wf_glob Σ -> optimize_env Σ = optimize_env' Σ.(GlobalContextMap.global_decls) Σ.(GlobalContextMap.wf).
+Lemma unbox_env_eq {efl : EEnvFlags} (Σ : GlobalContextMap.t) : wf_glob Σ -> unbox_env Σ = unbox_env' Σ.(GlobalContextMap.global_decls) Σ.(GlobalContextMap.wf).
 Proof.
   intros wf.
   now apply (gen_transform_env_eq (gt := GTExt efl)).
 Qed.
 
-Lemma optimize_env_expanded {efl : EEnvFlags} {Σ : GlobalContextMap.t} :
-  wf_glob Σ -> expanded_global_env Σ -> expanded_global_env (optimize_env Σ).
+Lemma unbox_env_expanded {efl : EEnvFlags} {Σ : GlobalContextMap.t} :
+  wf_glob Σ -> expanded_global_env Σ -> expanded_global_env (unbox_env Σ).
 Proof.
   unfold expanded_global_env; move=> wfg.
-  rewrite optimize_env_eq //.
+  rewrite unbox_env_eq //.
   destruct Σ as [Σ map repr wf]. cbn in *.
   clear map repr.
   induction 1; cbn; constructor; auto.
   cbn in IHexpanded_global_declarations.
   unshelve eapply IHexpanded_global_declarations. now depelim wfg. cbn.
   set (Σ' := GlobalContextMap.make _ _).
-  rewrite -(optimize_env_eq Σ'). cbn. now depelim wfg.
-  eapply (optimize_expanded_decl_irrel (Σ := Σ')). now depelim wfg.
-  now unshelve eapply (optimize_expanded_decl (Σ:=Σ')).
+  rewrite -(unbox_env_eq Σ'). cbn. now depelim wfg.
+  eapply (unbox_expanded_decl_irrel (Σ := Σ')). now depelim wfg.
+  now unshelve eapply (unbox_expanded_decl (Σ:=Σ')).
 Qed.
 
 Lemma Pre_glob efl Σ wf :
@@ -2237,36 +2207,37 @@ Proof.
   split => //. destruct d as [[[|]]|] => //=.
 Qed.
 
-Lemma optimize_env_wf {efl : EEnvFlags} {Σ : GlobalContextMap.t} :
+Lemma unbox_env_wf {efl : EEnvFlags} {Σ : GlobalContextMap.t} :
   has_tBox -> has_tRel ->
-  wf_glob Σ -> wf_glob (efl := disable_projections_env_flag efl) (optimize_env Σ).
+  wf_glob Σ -> wf_glob (efl := disable_projections_env_flag efl) (unbox_env Σ).
 Proof.
   intros hasb hasre wfg.
   eapply (gen_transform_env_wf (gt := GTExt efl)) => //.
   now apply Pre_glob.
 Qed.
 
-Definition optimize_program (p : eprogram_env) :=
-  (optimize_env p.1, optimize p.1 p.2).
+Definition unbox_program (p : eprogram_env) :=
+  (unbox_env p.1, unbox p.1 p.2).
 
-Definition optimize_program_wf {efl : EEnvFlags} (p : eprogram_env) {hastbox : has_tBox} {hastrel : has_tRel} :
-  wf_eprogram_env efl p -> wf_eprogram (disable_projections_env_flag efl) (optimize_program p).
+Definition unbox_program_wf {efl : EEnvFlags} (p : eprogram_env) {hastbox : has_tBox} {hastrel : has_tRel} :
+  wf_eprogram_env efl p -> wf_eprogram (disable_projections_env_flag efl) (unbox_program p).
 Proof.
   intros []; split.
-  now eapply optimize_env_wf.
-  cbn. now eapply optimize_wellformed.
+  now eapply unbox_env_wf.
+  cbn. now eapply unbox_wellformed.
 Qed.
 
-Definition optimize_program_expanded {efl} (p : eprogram_env) :
+Definition unbox_program_expanded {efl} (p : eprogram_env) :
   wf_eprogram_env efl p ->
-  expanded_eprogram_env_cstrs p -> expanded_eprogram_cstrs (optimize_program p).
+  expanded_eprogram_env_cstrs p -> expanded_eprogram_cstrs (unbox_program p).
 Proof.
   unfold expanded_eprogram_env_cstrs.
   move=> [wfe wft] /andP[] etae etat.
   apply/andP; split.
-  cbn. eapply expanded_global_env_isEtaExp_env, optimize_env_expanded => //.
+  cbn. eapply expanded_global_env_isEtaExp_env, unbox_env_expanded => //.
   now eapply isEtaExp_env_expanded_global_env.
   eapply expanded_isEtaExp.
-  eapply optimize_expanded_irrel => //.
-  now apply optimize_expanded, isEtaExp_expanded.
+  eapply unbox_expanded_irrel => //.
+  now apply unbox_expanded, isEtaExp_expanded.
 Qed.
+*)
