erasure-plugin/theories/Erasure.v
@@ -95,16 +95,17 @@ Definition final_wcbv_flags := {|
   with_constructor_as_block := true |}.
 
 Program Definition optional_unsafe_transforms econf :=
+  let efl := EConstructorsAsBlocks.switch_cstr_as_blocks
+  (EInlineProjections.disable_projections_env_flag (ERemoveParams.switch_no_params EWellformed.all_env_flags)) in
   ETransform.optional_self_transform econf.(enable_cofix_to_fix)
     ((* Rebuild the efficient lookup table *)
-    rebuild_wf_env_transform (efl := EConstructorsAsBlocks.switch_cstr_as_blocks
-      (EInlineProjections.disable_projections_env_flag (ERemoveParams.switch_no_params EWellformed.all_env_flags))) false false ▷
+    rebuild_wf_env_transform (efl := efl) false false ▷
     (* Coinductives & cofixpoints are translated to inductive types and thunked fixpoints *)
-    let efl := EConstructorsAsBlocks.switch_cstr_as_blocks
-      (EInlineProjections.disable_projections_env_flag (ERemoveParams.switch_no_params EWellformed.all_env_flags)) in
     coinductive_to_inductive_transformation efl
       (has_app := eq_refl) (has_box := eq_refl) (has_rel := eq_refl) (has_pars := eq_refl) (has_cstrblocks := eq_refl) ▷
-    reorder_cstrs_transformation efl final_wcbv_flags econf.(inductives_mapping)).
+    reorder_cstrs_transformation efl final_wcbv_flags econf.(inductives_mapping) ▷
+    rebuild_wf_env_transform (efl := efl) false false ▷
+    unbox_transformation efl final_wcbv_flags).
 
 Program Definition verified_lambdabox_pipeline {guard : abstract_guard_impl}
   (efl := EWellformed.all_env_flags)
